POPL24

coq/theories/erasure_subst.v
@@ -1,50 +1,54 @@
+(* This file presents the program substitution lemmas instrumented
+   to cover the erasure procedure. *)
+
 From mathcomp Require Import ssreflect ssrbool eqtype ssrnat seq.
 From Coq Require Import ssrfun Classical Utf8.
-Require Export AutosubstSsr ARS era_weak.
+Require Export AutosubstSsr ARS erasure_weak.
 
 Set Implicit Arguments.
 Unset Strict Implicit.
 Unset Printing Implicit Defensive.
 
+(* Relation to strengthen induction for simultaneous substitution. *)
 Reserved Notation "Γ1 ; Δ1 ⊢ σ1 ~ σ2 ⊣ Γ2 ; Δ2"
   (at level 50, Δ1, σ1, σ2, Γ2 at next level).
-Inductive era_agree_subst :
-  sta_ctx -> dyn_ctx -> (var -> term) -> (var -> term) -> sta_ctx -> dyn_ctx -> Prop :=
-| era_agree_subst_nil σ :
+Inductive erasure_agree_subst :
+  logical_ctx -> program_ctx -> (var -> term) -> (var -> term) -> logical_ctx -> program_ctx -> Prop :=
+| erasure_agree_subst_nil σ :
   nil ; nil ⊢ σ ~ σ ⊣ nil ; nil
-| era_agree_subst_ty Γ1 Δ1 σ1 σ2 Γ2 Δ2 A s :
+| erasure_agree_subst_ty Γ1 Δ1 σ1 σ2 Γ2 Δ2 A s :
   Γ1 ; Δ1 ⊢ σ1 ~ σ2 ⊣ Γ2 ; Δ2 ->
   Γ2 ⊢ A : Sort s ->
   (A.[σ1] :: Γ1) ; (A.[σ1] :{s} Δ1) ⊢ up σ1 ~ up σ2 ⊣ (A :: Γ2) ; (A :{s} Δ2)
-| era_agree_subst_n Γ1 Δ1 σ1 σ2 Γ2 Δ2 A s :
+| erasure_agree_subst_n Γ1 Δ1 σ1 σ2 Γ2 Δ2 A s :
   Γ1 ; Δ1 ⊢ σ1 ~ σ2 ⊣ Γ2 ; Δ2 ->
   Γ2 ⊢ A : Sort s ->
   (A.[σ1] :: Γ1) ; (_: Δ1) ⊢ up σ1 ~ up σ2 ⊣ (A :: Γ2) ; (_: Δ2)
-| era_agree_subst_wk0 Γ1 Δ1 σ1 σ2 Γ2 Δ2 n n' A :
+| erasure_agree_subst_wk0 Γ1 Δ1 σ1 σ2 Γ2 Δ2 n n' A :
   Γ1 ; Δ1 ⊢ σ1 ~ σ2 ⊣ Γ2 ; Δ2 ->
   Γ1 ⊢ n : A.[σ1] ->
   Γ1 ; Δ1 ⊢ n .: σ1 ~ n' .: σ2 ⊣ (A :: Γ2) ; (_: Δ2)
-| era_agree_subst_wk1 Γ1 Γ2 σ1 σ2 Δ1 Δ2 Δa Δb n n' A s :
+| erasure_agree_subst_wk1 Γ1 Γ2 σ1 σ2 Δ1 Δ2 Δa Δb n n' A s :
   Δb ▷ s ->
   Δa ∘ Δb => Δ1 ->
   Γ1 ; Δa ⊢ σ1 ~ σ2 ⊣ Γ2 ; Δ2 ->
   Γ1 ; Δb ⊢ n ~ n' : A.[σ1] ->
   Γ1 ; Δ1 ⊢ n .: σ1 ~ n' .: σ2 ⊣ (A :: Γ2) ; (A :{s} Δ2)
-| era_agree_subst_conv0 Γ1 Δ1 σ1 σ2 Γ2 Δ2 A B s :
+| erasure_agree_subst_conv0 Γ1 Δ1 σ1 σ2 Γ2 Δ2 A B s :
   A === B ->
   Γ1 ⊢ B.[ren (+1)].[σ1] : Sort s ->
   Γ2 ⊢ B : Sort s ->
   Γ1 ; Δ1 ⊢ σ1 ~ σ2 ⊣ (A :: Γ2) ; (_: Δ2) ->
   Γ1 ; Δ1 ⊢ σ1 ~ σ2 ⊣ (B :: Γ2) ; (_: Δ2)
-| era_agree_subst_conv1 Γ1 Δ1 σ1 σ2 Γ2 Δ2 A B s :
+| erasure_agree_subst_conv1 Γ1 Δ1 σ1 σ2 Γ2 Δ2 A B s :
   A === B ->
   Γ1 ⊢ B.[ren (+1)].[σ1] : Sort s ->
   Γ2 ⊢ B : Sort s ->
   Γ1 ; Δ1 ⊢ σ1 ~ σ2 ⊣ (A :: Γ2) ; (A :{s} Δ2) ->
   Γ1 ; Δ1 ⊢ σ1 ~ σ2 ⊣ (B :: Γ2) ; (B :{s} Δ2)
-where "Γ1 ; Δ1 ⊢ σ1 ~ σ2 ⊣ Γ2 ; Δ2" := (era_agree_subst Γ1 Δ1 σ1 σ2 Γ2 Δ2).
+where "Γ1 ; Δ1 ⊢ σ1 ~ σ2 ⊣ Γ2 ; Δ2" := (erasure_agree_subst Γ1 Δ1 σ1 σ2 Γ2 Δ2).
 
-Lemma era_agree_subst_key Γ1 Γ2 Δ1 Δ2 σ1 σ2 s :
+Lemma erasure_agree_subst_key Γ1 Γ2 Δ1 Δ2 σ1 σ2 s :
   Γ1 ; Δ1 ⊢ σ1 ~ σ2 ⊣ Γ2 ; Δ2 -> Δ2 ▷ s -> Δ1 ▷ s.
 Proof with eauto using key.
   move=>agr. elim: agr s=>{Γ1 Γ2 Δ1 Δ2 σ1 σ2}...
@@ -56,20 +60,20 @@ Proof with eauto using key.
   { move=>Γ1 Δ1 σ1 σ2 Γ2 Δ2 A B s eq tyB1 tyB2 agr ih r k. inv k... }
 Qed.
 
-Lemma era_dyn_agree_subst Γ1 Γ2 Δ1 Δ2 σ1 σ2 :
+Lemma erasure_program_agree_subst Γ1 Γ2 Δ1 Δ2 σ1 σ2 :
   Γ1 ; Δ1 ⊢ σ1 ~ σ2 ⊣ Γ2 ; Δ2 -> Γ1 ; Δ1 ⊢ σ1 ⊣ Γ2 ; Δ2.
-Proof with eauto using dyn_agree_subst.
+Proof with eauto using program_agree_subst.
   elim=>{Γ1 Γ2 Δ1 Δ2 σ1 σ2}...
 Qed.
 
-Lemma era_sta_agree_subst Γ1 Γ2 Δ1 Δ2 σ1 σ2 :
+Lemma erasure_logical_agree_subst Γ1 Γ2 Δ1 Δ2 σ1 σ2 :
   Γ1 ; Δ1 ⊢ σ1 ~ σ2 ⊣ Γ2 ; Δ2 -> Γ1 ⊢ σ1 ⊣ Γ2.
-Proof with eauto using sta_agree_subst.
-  move/era_dyn_agree_subst/dyn_sta_agree_subst=>//.
+Proof with eauto using logical_agree_subst.
+  move/erasure_program_agree_subst/program_logical_agree_subst=>//.
 Qed.
 
-Lemma era_agree_subst_refl Γ Δ : dyn_wf Γ Δ -> Γ ; Δ ⊢ ids ~ ids ⊣ Γ ; Δ.
-Proof with eauto using era_agree_subst.
+Lemma erasure_agree_subst_refl Γ Δ : program_wf Γ Δ -> Γ ; Δ ⊢ ids ~ ids ⊣ Γ ; Δ.
+Proof with eauto using erasure_agree_subst.
   elim: Γ Δ.
   { move=>Δ wf. inv wf... }
   { move=>A Γ ih Δ wf. inv wf.
@@ -81,37 +85,37 @@ Proof with eauto using era_agree_subst.
       have:(A.[ids] :: Γ); _: Δ0 ⊢ up ids ~ up ids ⊣ (A :: Γ); _: Δ0...
       by asimpl. } }
 Qed.
-#[global] Hint Resolve era_agree_subst_refl.
+#[global] Hint Resolve erasure_agree_subst_refl.
 
-Lemma era_agree_subst_has Γ1 Γ2 σ1 σ2 Δ1 Δ2 x s A :
-  Γ1 ; Δ1 ⊢ σ1 ~ σ2 ⊣ Γ2 ; Δ2 -> dyn_wf Γ1 Δ1 -> dyn_has Δ2 x s A ->
+Lemma erasure_agree_subst_has Γ1 Γ2 σ1 σ2 Δ1 Δ2 x s A :
+  Γ1 ; Δ1 ⊢ σ1 ~ σ2 ⊣ Γ2 ; Δ2 -> program_wf Γ1 Δ1 -> program_has Δ2 x s A ->
   Γ1 ; Δ1 ⊢ (σ1 x) ~ (σ2 x) : A.[σ1].
-Proof with eauto using era_agree_subst, era_agree_subst_key.
+Proof with eauto using erasure_agree_subst, erasure_agree_subst_key.
   move=>agr. elim: agr x s A=>{Γ1 Γ2 σ1 σ2 Δ1 Δ2}...
   { move=>σ x s A wf hs. inv hs. }
   { move=>Γ1 Δ1 σ1 σ2 Γ2 Δ2 A s agr ih tyA x t B wf hs.
     inv wf. inv hs; asimpl.
     replace A.[σ1 >> ren (+1)] with A.[σ1].[ren (+1)] by autosubst.
-    apply: era_var; constructor...
+    apply: erasure_var; constructor...
     replace A0.[σ1 >> ren (+1)] with A0.[σ1].[ren (+1)] by autosubst.
-    apply: era_eweakenU... }
+    apply: erasure_eweaken1... }
   { move=>Γ1 Δ1 σ1 σ2 Γ2 Δ2 A s agr ih tyA x t B wf hs.
     inv wf. inv hs; asimpl...
     replace A0.[σ1 >> ren (+1)] with A0.[σ1].[ren (+1)]
       by autosubst.
-    apply: era_eweakenN... }
+    apply: erasure_eweaken0... }
   { move=>Γ1 Δ1 σ1 σ2 Γ2 Δ2 n n' A agr ih tyn x t B wf hs. inv hs; asimpl... }
   { move=>Γ1 Γ2 σ1 σ2 Δ1 Δ2 Δa Δb n n' A s k mrg agr ih tyn x t B wf hs.
     inv hs; asimpl.
-    { have ka:=era_agree_subst_key agr H5.
+    { have ka:=erasure_agree_subst_key agr H5.
       have->//:=merge_pureL mrg ka. }
     { have->:=merge_pureR mrg k.
       apply: ih...
-      have[]//:=dyn_wf_inv mrg wf. } }
+      have[]//:=program_wf_inv mrg wf. } }
   { move=>Γ1 Δ1 σ1 σ2 Γ2 Δ2 A B s eq tyB1 tyB2 agr ih x t C wf hs. inv hs.
-    { apply: era_conv.
-      apply: sta_conv_subst.
-      apply: sta_conv_subst...
+    { apply: erasure_conv.
+      apply: logical_conv_subst.
+      apply: logical_conv_subst...
       apply: ih...
       constructor...
       exact: tyB1. }
@@ -119,12 +123,12 @@ Proof with eauto using era_agree_subst, era_agree_subst_key.
       constructor... } }
 Qed.
 
-Lemma era_agree_subst_merge Γ1 Γ2 Δ1 Δ2 Δa Δb σ1 σ2 :
+Lemma erasure_agree_subst_merge Γ1 Γ2 Δ1 Δ2 Δa Δb σ1 σ2 :
   Γ1 ; Δ1 ⊢ σ1 ~ σ2 ⊣ Γ2 ; Δ2 -> Δa ∘ Δb => Δ2 ->
   exists Δa' Δb',
     Δa' ∘ Δb' => Δ1 /\
     Γ1 ; Δa' ⊢ σ1 ~ σ2 ⊣ Γ2 ; Δa /\ Γ1 ; Δb' ⊢ σ1 ~ σ2 ⊣ Γ2 ; Δb.
-Proof with eauto 6 using merge, era_agree_subst, era_agree_subst_key.
+Proof with eauto 6 using merge, erasure_agree_subst, erasure_agree_subst_key.
   move=>agr. elim: agr Δa Δb=>{Γ1 Γ2 Δ1 Δ2 σ1 σ2}.
   { move=>σ Δa Δb mrg. inv mrg.
     exists nil. exists nil... }
@@ -147,7 +151,7 @@ Proof with eauto 6 using merge, era_agree_subst, era_agree_subst_key.
       have[Δc[mrg1 mrg2]]:=merge_splitL mrg mrg'.
       exists Δc. exists Δb'.
       repeat split...
-      apply: era_agree_subst_wk1...
+      apply: erasure_agree_subst_wk1...
       have[Δd[mrg3 mrg4]]:=merge_splitR mrg mrg'.
       have e:=merge_pureR mrg3 k.
       by subst. }
@@ -172,79 +176,80 @@ Proof with eauto 6 using merge, era_agree_subst, era_agree_subst_key.
       exists Δa'. exists Δb'... } }
 Qed.
 
-Lemma era_substitution Γ1 Γ2 m m' A Δ1 Δ2 σ1 σ2 :
+(* Simultaneous substitution lemma. *)
+Lemma erasure_substitution Γ1 Γ2 m m' A Δ1 Δ2 σ1 σ2 :
   Γ2 ; Δ2 ⊢ m ~ m' : A -> Γ1 ; Δ1 ⊢ σ1 ~ σ2 ⊣ Γ2 ; Δ2 ->
   Γ1 ; Δ1 ⊢ m.[σ1] ~ m'.[σ2] : A.[σ1].
-Proof with eauto using era_agree_subst, era_agree_subst_key, era_type.
+Proof with eauto using erasure_agree_subst, erasure_agree_subst_key, erasure_type.
   move=>ty. elim: ty Γ1 Δ1 σ1 σ2=>{Γ2 Δ2 m m' A}.
   { move=>Γ Δ x s A wf shs dhs Γ1 Δ1 σ1 σ2 agr. asimpl.
-    apply: era_agree_subst_has...
-    apply: dyn_substitution_wf...
-    apply: era_dyn_agree_subst... }
+    apply: erasure_agree_subst_has...
+    apply: program_substitution_wf...
+    apply: erasure_program_agree_subst... }
   { move=>Γ Δ A B m m' s k tym ihm Γ1 Δ1 σ1 σ2 agr. asimpl.
-    have wf:=dyn_type_wf (era_dyn_type tym). inv wf.
-    apply: era_lam0... }
+    have wf:=program_type_wf (erasure_program_reflect tym). inv wf.
+    apply: erasure_lam0... }
   { move=>Γ Δ A B m m' s t k tym ihm Γ1 Δ1 σ1 σ2 agr. asimpl.
-    have wf:=dyn_type_wf (era_dyn_type tym). inv wf.
-    apply: era_lam1... }
+    have wf:=program_type_wf (erasure_program_reflect tym). inv wf.
+    apply: erasure_lam1... }
   { move=>Γ Δ A B m m' n s tym ihm tyn Γ1 Δ1 σ1 σ2 agr. asimpl.
     replace B.[n.[σ1] .: σ1] with B.[up σ1].[n.[σ1]/] by autosubst.
     have{}ihm:=ihm _ _ _ _ agr.
-    apply: era_app0...
-    have//:=sta_substitution tyn (era_sta_agree_subst agr). }
+    apply: erasure_app0...
+    have//:=logical_substitution tyn (erasure_logical_agree_subst agr). }
   { move=>Γ Δ1 Δ2 Δ A B m m' n n' s mrg tym ihm tyn ihn
       Γ1 Δ0 σ1 σ2 agr. asimpl.
     replace B.[n.[σ1] .: σ1] with B.[up σ1].[n.[σ1]/] by autosubst.
-    have[Δa[Δb[mrg0[agra agrb]]]]:=era_agree_subst_merge agr mrg.
+    have[Δa[Δb[mrg0[agra agrb]]]]:=erasure_agree_subst_merge agr mrg.
     have{}ihm:=ihm _ _ _ _ agra.
     have{}ihn:=ihn _ _ _ _ agrb.
-    apply: era_app1... }
+    apply: erasure_app1... }
   { move=>Γ Δ A B m m' n t tyS tym ihm tyn Γ1 Δ1 σ1 σ2 agr. asimpl.
-    have{}ihS:=sta_substitution tyS (dyn_sta_agree_subst (era_dyn_agree_subst agr)).
+    have{}ihS:=logical_substitution tyS (program_logical_agree_subst (erasure_program_agree_subst agr)).
     have{}ihm:=ihm _ _ _ _ agr.
-    have{}ihn:=sta_substitution tyn (dyn_sta_agree_subst (era_dyn_agree_subst agr)).
-    apply: era_pair0...
+    have{}ihn:=logical_substitution tyn (program_logical_agree_subst (erasure_program_agree_subst agr)).
+    apply: erasure_pair0...
     asimpl. asimpl in ihn... }
   { move=>Γ Δ1 Δ2 Δ A B m m' n n' t mrg tyS tym ihm tyn ihn Γ1 Δ0 σ1 σ2 agr. asimpl.
-    have[Δa[Δb[mrg0[agra agrb]]]]:=era_agree_subst_merge agr mrg.
-    have{}ihS:=sta_substitution tyS (dyn_sta_agree_subst (era_dyn_agree_subst agr)).
+    have[Δa[Δb[mrg0[agra agrb]]]]:=erasure_agree_subst_merge agr mrg.
+    have{}ihS:=logical_substitution tyS (program_logical_agree_subst (erasure_program_agree_subst agr)).
     have{}ihm:=ihm _ _ _ _ agra.
     have{}ihn:=ihn _ _ _ _ agrb.
-    apply: era_pair1...
+    apply: erasure_pair1...
     asimpl. asimpl in ihn... }
   { move=>Γ Δ1 Δ2 Δ A B C m m' n n' s r t mrg tyC tym ihm tyn ihn Γ1 Δ0 σ1 σ2 agr. asimpl.
-    have[Δa[Δb[mrg0[agra agrb]]]]:=era_agree_subst_merge agr mrg.
+    have[Δa[Δb[mrg0[agra agrb]]]]:=erasure_agree_subst_merge agr mrg.
     replace C.[m.[σ1] .: σ1] with C.[up σ1].[m.[σ1]/] by autosubst.
-    have wf:=sta_type_wf tyC. inv wf.
-    have wf:=dyn_type_wf (era_dyn_type tyn). inv wf. inv H4.
-    have{}ihC:=sta_substitution tyC
-      (sta_agree_subst_ty (dyn_sta_agree_subst (era_dyn_agree_subst agr)) H2).
+    have wf:=logical_type_wf tyC. inv wf.
+    have wf:=program_type_wf (erasure_program_reflect tyn). inv wf. inv H4.
+    have{}ihC:=logical_substitution tyC
+      (logical_agree_subst_ty (program_logical_agree_subst (erasure_program_agree_subst agr)) H2).
     have{}ihm:=ihm _ _ _ _ agra.
-    have{}ihn:=ihn _ _ _ _ (era_agree_subst_n (era_agree_subst_ty agrb H8) H5).
-    apply: era_letin0...
+    have{}ihn:=ihn _ _ _ _ (erasure_agree_subst_n (erasure_agree_subst_ty agrb H8) H5).
+    apply: erasure_letin0...
     asimpl. asimpl in ihn... }
   { move=>Γ Δ1 Δ2 Δ A B C m m' n n' s r1 r2 t mrg tyC tym ihm tyn ihn Γ1 Δ0 σ1 σ2 agr. asimpl.
-    have[Δa[Δb[mrg0[agra agrb]]]]:=era_agree_subst_merge agr mrg.
+    have[Δa[Δb[mrg0[agra agrb]]]]:=erasure_agree_subst_merge agr mrg.
     replace C.[m.[σ1] .: σ1] with C.[up σ1].[m.[σ1]/] by autosubst.
-    have wf:=sta_type_wf tyC. inv wf.
-    have wf:=dyn_type_wf (era_dyn_type tyn). inv wf. inv H4.
-    have{}ihC:=sta_substitution tyC
-      (sta_agree_subst_ty (dyn_sta_agree_subst (era_dyn_agree_subst agr)) H2).
+    have wf:=logical_type_wf tyC. inv wf.
+    have wf:=program_type_wf (erasure_program_reflect tyn). inv wf. inv H4.
+    have{}ihC:=logical_substitution tyC
+      (logical_agree_subst_ty (program_logical_agree_subst (erasure_program_agree_subst agr)) H2).
     have{}ihm:=ihm _ _ _ _ agra.
-    have{}ihn:=ihn _ _ _ _ (era_agree_subst_ty (era_agree_subst_ty agrb H8) H6).
-    apply: era_letin1...
+    have{}ihn:=ihn _ _ _ _ (erasure_agree_subst_ty (erasure_agree_subst_ty agrb H8) H6).
+    apply: erasure_letin1...
     asimpl. asimpl in ihn... }
-  { move=>Γ Δ A B m m' n n' t k tym ihm tyn ihn Γ1 Δ1 σ1 σ2 agr. asimpl. apply: era_apair... }
-  { move=>Γ Δ A B m m' t tym ihm Γ1 Δ1 σ1 σ2 agr. asimpl. apply: era_fst... }
-  { move=>Γ Δ A B m m' t tym ihm Γ1 Δ1 σ1 σ2 agr. asimpl. apply: era_snd... }
+  { move=>Γ Δ A B m m' n n' t k tym ihm tyn ihn Γ1 Δ1 σ1 σ2 agr. asimpl. apply: erasure_apair... }
+  { move=>Γ Δ A B m m' t tym ihm Γ1 Δ1 σ1 σ2 agr. asimpl. apply: erasure_fst... }
+  { move=>Γ Δ A B m m' t tym ihm Γ1 Δ1 σ1 σ2 agr. asimpl. apply: erasure_snd... }
   { move=>Γ Δ A B H H' P m n s tyB erH ihH tyP Γ1 Δ1 σ1 σ2 agr. asimpl.
     replace B.[P.[σ1] .: n.[σ1] .: σ1] with B.[upn 2 σ1].[P.[σ1],n.[σ1]/] by autosubst.
-    have wf:=sta_type_wf tyB. inv wf. inv H2.
-    have agr':=era_sta_agree_subst agr.
-    have ihB:=sta_substitution tyB (sta_agree_subst_ty (sta_agree_subst_ty agr' H5) H3).
-    have ihP:=sta_substitution tyP agr'.
+    have wf:=logical_type_wf tyB. inv wf. inv H2.
+    have agr':=erasure_logical_agree_subst agr.
+    have ihB:=logical_substitution tyB (logical_agree_subst_ty (logical_agree_subst_ty agr' H5) H3).
+    have ihP:=logical_substitution tyP agr'.
     have{}ihH:=ihH _ _ _ _ agr.
-    apply: era_rw.
+    apply: erasure_rw.
     asimpl in ihB.
     replace A.[σ1 >> ren (+1)] with A.[σ1].[ren (+1)] in ihB by autosubst.
     replace m.[σ1 >> ren (+1)] with m.[σ1].[ren (+1)] in ihB by autosubst.
@@ -252,45 +257,49 @@ Proof with eauto using era_agree_subst, era_agree_subst_key, era_type.
     asimpl. asimpl in ihH...
     asimpl in ihP... }
   { move=>Γ Δ A B m m' s eq tym ihm tyB Γ1 Δ1 σ1 σ2 agr.
-    apply: era_conv.
-    apply: sta_conv_subst...
+    apply: erasure_conv.
+    apply: logical_conv_subst...
     apply: ihm...
-    have:=sta_substitution tyB (era_sta_agree_subst agr).
+    have:=logical_substitution tyB (erasure_logical_agree_subst agr).
     asimpl... }
 Qed.
 
-Lemma era_subst0 Γ Δ m m' n A B :
+(* Program 0-Substitution instrumented for erasure. *)
+Lemma erasure_subst0 Γ Δ m m' n A B :
   (A :: Γ) ; _: Δ ⊢ m ~ m' : B -> Γ ⊢ n : A -> Γ ; Δ ⊢ m.[n/] ~ m'.[Box/] : B.[n/].
-Proof with eauto using era_agree_subst_refl.
+Proof with eauto using erasure_agree_subst_refl.
   move=>tym tyn.
-  have wf:=dyn_type_wf (era_dyn_type tym). inv wf.
-  apply: era_substitution...
-  apply: era_agree_subst_wk0...
+  have wf:=program_type_wf (erasure_program_reflect tym). inv wf.
+  apply: erasure_substitution...
+  apply: erasure_agree_subst_wk0...
   by asimpl.
 Qed.
 
-Lemma era_subst1 Γ Δ1 Δ2 Δ m m' n n' A B s :
+(* Program 1-Substitution instrumented for erasure. *)
+Lemma erasure_subst1 Γ Δ1 Δ2 Δ m m' n n' A B s :
   Δ2 ▷ s -> Δ1 ∘ Δ2 => Δ ->
   (A :: Γ) ; A :{s} Δ1 ⊢ m ~ m' : B -> Γ ; Δ2 ⊢ n ~ n' : A -> Γ ; Δ ⊢ m.[n/] ~ m'.[n'/] : B.[n/].
-Proof with eauto using era_agree_subst_refl.
+Proof with eauto using erasure_agree_subst_refl.
   move=>k mrg tym tyn.
-  have wf:=dyn_type_wf (era_dyn_type tym). inv wf.
-  apply: era_substitution...
-  apply: era_agree_subst_wk1...
+  have wf:=program_type_wf (erasure_program_reflect tym). inv wf.
+  apply: erasure_substitution...
+  apply: erasure_agree_subst_wk1...
   by asimpl.
 Qed.
 
-Lemma era_esubst0 Γ Δ m m' n n' v A B B' :
+(* Alternative statement more suitable for certain Coq tactics *)
+Lemma erasure_esubst0 Γ Δ m m' n n' v A B B' :
   m' = m.[v/] ->
   n' = n.[Box/] ->
   B' = B.[v/] ->
   (A :: Γ) ; _: Δ ⊢ m ~ n : B -> Γ ⊢ v : A ->
   Γ ; Δ ⊢ m' ~ n' : B'.
 Proof.
-  move=>*; subst. apply: era_subst0; eauto.
+  move=>*; subst. apply: erasure_subst0; eauto.
 Qed.
 
-Lemma era_esubst1 Γ Δ1 Δ2 Δ m m' n n' v v' A B B' s :
+(* Alternative statement more suitable for certain Coq tactics *)
+Lemma erasure_esubst1 Γ Δ1 Δ2 Δ m m' n n' v v' A B B' s :
   m' = m.[v/] ->
   n' = n.[v'/] ->
   B' = B.[v/] ->
@@ -299,34 +308,36 @@ Lemma era_esubst1 Γ Δ1 Δ2 Δ m m' n n' v v' A B B' s :
   Γ ; Δ2 ⊢ v ~ v' : A ->
   Γ ; Δ ⊢ m' ~ n' : B'.
 Proof.
-  move=>*; subst. apply: era_subst1; eauto.
+  move=>*; subst. apply: erasure_subst1; eauto.
 Qed.
 
-Lemma era_ctx_conv0 Γ Δ m m' A B C s :
+(* Instrumented context conversion lemma for the logical context. *)
+Lemma erasure_ctx_conv0 Γ Δ m m' A B C s :
   B === A ->
   Γ ⊢ B : Sort s -> (A :: Γ) ; _: Δ ⊢ m ~ m' : C -> (B :: Γ) ; _: Δ ⊢ m ~ m' : C.
-Proof with eauto using dyn_wf, era_agree_subst_refl.
+Proof with eauto using program_wf, erasure_agree_subst_refl.
   move=>eq tyB tym.
-  have wf:=dyn_type_wf (era_dyn_type tym). inv wf.
+  have wf:=program_type_wf (erasure_program_reflect tym). inv wf.
   have:(B :: Γ) ; _: Δ ⊢ m.[ids] ~ m'.[ids] : C.[ids].
-  apply: era_substitution...
-  apply: era_agree_subst_conv0...
-  apply: sta_eweaken...
+  apply: erasure_substitution...
+  apply: erasure_agree_subst_conv0...
+  apply: logical_eweaken...
   asimpl...
   asimpl...
   asimpl...
 Qed.
 
-Lemma era_ctx_conv1 Γ Δ m m' A B C s :
+(* Instrumented context conversion lemma for the program context. *)
+Lemma erasure_ctx_conv1 Γ Δ m m' A B C s :
   B === A ->
   Γ ⊢ B : Sort s -> (A :: Γ) ; A :{s} Δ ⊢ m ~ m' : C -> (B :: Γ) ; B :{s} Δ ⊢ m ~ m' : C.
-Proof with eauto using dyn_wf, era_agree_subst_refl.
+Proof with eauto using program_wf, erasure_agree_subst_refl.
   move=>eq tyA tym.
-  have wf:=dyn_type_wf (era_dyn_type tym). inv wf.
+  have wf:=program_type_wf (erasure_program_reflect tym). inv wf.
   have:(B :: Γ) ; B :{s} Δ ⊢ m.[ids] ~ m'.[ids] : C.[ids].
-  apply: era_substitution...
-  apply: era_agree_subst_conv1...
-  apply: sta_eweaken...
+  apply: erasure_substitution...
+  apply: erasure_agree_subst_conv1...
+  apply: logical_eweaken...
   asimpl...
   asimpl...
   asimpl...
