coq/theories/program_step.v
@@ -6,69 +6,69 @@ Set Implicit Arguments.
 Unset Strict Implicit.
 Unset Printing Implicit Defensive.
 
-Inductive dyn_val : term -> Prop :=
-| dyn_val_var x :
-  dyn_val (Var x)
-| dyn_val_lam0 A B s :
-  dyn_val (Lam0 A B s)
-| dyn_val_lam1 A B s :
-  dyn_val (Lam1 A B s)
-| dyn_val_pair0 m1 m2 s :
-  dyn_val m1 ->
-  dyn_val (Pair0 m1 m2 s)
-| dyn_val_pair1 m1 m2 s :
-  dyn_val m1 ->
-  dyn_val m2 ->
-  dyn_val (Pair1 m1 m2 s)
-| dyn_val_apair m1 m2 s :
-  dyn_val (APair m1 m2 s)
-| dyn_val_ptr l :
-  dyn_val (Ptr l).
+Inductive program_val : term -> Prop :=
+| program_val_var x :
+  program_val (Var x)
+| program_val_lam0 A B s :
+  program_val (Lam0 A B s)
+| program_val_lam1 A B s :
+  program_val (Lam1 A B s)
+| program_val_pair0 m1 m2 s :
+  program_val m1 ->
+  program_val (Pair0 m1 m2 s)
+| program_val_pair1 m1 m2 s :
+  program_val m1 ->
+  program_val m2 ->
+  program_val (Pair1 m1 m2 s)
+| program_val_apair m1 m2 s :
+  program_val (APair m1 m2 s)
+| program_val_ptr l :
+  program_val (Ptr l).
 
 Reserved Notation "m ~>> n" (at level 50).
-Inductive dyn_step : term -> term -> Prop :=
-| dyn_step_appL m m' n :
+Inductive program_step : term -> term -> Prop :=
+| program_step_appL m m' n :
   m ~>> m' ->
   App m n ~>> App m' n
-| dyn_step_appR m n n' :
+| program_step_appR m n n' :
   n ~>> n' ->
   App m n ~>> App m n'
-| dyn_step_beta0 A m n s :
+| program_step_beta0 A m n s :
   App (Lam0 A m s) n ~>> m.[n/]
-| dyn_step_beta1 A m v s :
-  dyn_val v ->
+| program_step_beta1 A m v s :
+  program_val v ->
   App (Lam1 A m s) v ~>> m.[v/]
-| dyn_step_pair0L m m' n s :
+| program_step_pair0L m m' n s :
   m ~>> m' ->
   Pair0 m n s ~>> Pair0 m' n s
-| dyn_step_pair1L m m' n s :
+| program_step_pair1L m m' n s :
   m ~>> m' ->
   Pair1 m n s ~>> Pair1 m' n s
-| dyn_step_pair1R m n n' s :
+| program_step_pair1R m n n' s :
   n ~>> n' ->
   Pair1 m n s ~>> Pair1 m n' s
-| dyn_step_letinL A m m' n :
+| program_step_letinL A m m' n :
   m ~>> m' ->
   LetIn A m n ~>> LetIn A m' n
-| dyn_step_iota0 A m1 m2 n s :
-  dyn_val (Pair0 m1 m2 s) ->
+| program_step_iota0 A m1 m2 n s :
+  program_val (Pair0 m1 m2 s) ->
   LetIn A (Pair0 m1 m2 s) n ~>> n.[m2,m1/]
-| dyn_step_iota1 A m1 m2 n s :
-  dyn_val (Pair1 m1 m2 s) ->
+| program_step_iota1 A m1 m2 n s :
+  program_val (Pair1 m1 m2 s) ->
   LetIn A (Pair1 m1 m2 s) n ~>> n.[m2,m1/]
-| dyn_step_fst m m' :
+| program_step_fst m m' :
   m ~>> m' ->
   Fst m ~>> Fst m'
-| dyn_step_snd m m' :
+| program_step_snd m m' :
   m ~>> m' ->
   Snd m ~>> Snd m'
-| dyn_step_proj1 m n s :
+| program_step_proj1 m n s :
   Fst (APair m n s) ~>> m
-| dyn_step_proj2 m n s :
+| program_step_proj2 m n s :
   Snd (APair m n s) ~>> n
-| dyn_step_rwE A H P :
+| program_step_rwE A H P :
   Rw A H P ~>> H
-where "m ~>> n" := (dyn_step m n).
+where "m ~>> n" := (program_step m n).
 
-Notation dyn_red := (star dyn_step).
-Notation "m ~>>* n" := (dyn_red m n) (at level 50).
+Notation program_red := (star program_step).
+Notation "m ~>>* n" := (program_red m n) (at level 50).
