coq/theories/program_subst.v
@@ -1,49 +1,52 @@
+(* This files presents the substitution lemmas for the program level. *)
+
 From mathcomp Require Import ssreflect ssrbool eqtype ssrnat seq.
 From Coq Require Import ssrfun Classical Utf8.
-Require Export AutosubstSsr ARS sta_subst sta_inv dyn_valid dyn_weak.
+Require Export AutosubstSsr ARS logical_subst logical_inv program_valid program_weak.
 
 Set Implicit Arguments.
 Unset Strict Implicit.
 Unset Printing Implicit Defensive.
 
+(* Relation to strengthen induction for simultaneous substitution. *)
 Reserved Notation "Γ1 ; Δ1 ⊢ σ ⊣ Γ2 ; Δ2" (at level 50, Δ1, σ, Γ2 at next level).
-Inductive dyn_agree_subst :
-  sta_ctx -> dyn_ctx -> (var -> term) -> sta_ctx -> dyn_ctx -> Prop :=
-| dyn_agree_subst_nil σ :
+Inductive program_agree_subst :
+  logical_ctx -> program_ctx -> (var -> term) -> logical_ctx -> program_ctx -> Prop :=
+| program_agree_subst_nil σ :
   nil ; nil ⊢ σ ⊣ nil ; nil
-| dyn_agree_subst_ty Γ1 Δ1 σ Γ2 Δ2 A s :
+| program_agree_subst_ty Γ1 Δ1 σ Γ2 Δ2 A s :
   Γ1 ; Δ1 ⊢ σ ⊣ Γ2 ; Δ2 ->
   Γ2 ⊢ A : Sort s ->
   (A.[σ] :: Γ1) ; (A.[σ] :{s} Δ1) ⊢ up σ ⊣ (A :: Γ2) ; (A :{s} Δ2)
-| dyn_agree_subst_n Γ1 Δ1 σ Γ2 Δ2 A s :
+| program_agree_subst_n Γ1 Δ1 σ Γ2 Δ2 A s :
   Γ1 ; Δ1 ⊢ σ ⊣ Γ2 ; Δ2 ->
   Γ2 ⊢ A : Sort s ->
   (A.[σ] :: Γ1) ; (_: Δ1) ⊢ up σ ⊣ (A :: Γ2) ; (_: Δ2)
-| dyn_agree_subst_wk0 Γ1 Δ1 σ Γ2 Δ2 n A :
+| program_agree_subst_wk0 Γ1 Δ1 σ Γ2 Δ2 n A :
   Γ1 ; Δ1 ⊢ σ ⊣ Γ2 ; Δ2 ->
   Γ1 ⊢ n : A.[σ] ->
   Γ1 ; Δ1 ⊢ n .: σ ⊣ (A :: Γ2) ; (_: Δ2)
-| dyn_agree_subst_wk1 Γ1 Γ2 σ Δ1 Δ2 Δa Δb n A s :
+| program_agree_subst_wk1 Γ1 Γ2 σ Δ1 Δ2 Δa Δb n A s :
   Δb ▷ s ->
   Δa ∘ Δb => Δ1 ->
   Γ1 ; Δa ⊢ σ ⊣ Γ2 ; Δ2 ->
   Γ1 ; Δb ⊢ n : A.[σ] ->
   Γ1 ; Δ1 ⊢ n .: σ ⊣ (A :: Γ2) ; (A :{s} Δ2)
-| dyn_agree_subst_conv0 Γ1 Δ1 σ Γ2 Δ2 A B s :
+| program_agree_subst_conv0 Γ1 Δ1 σ Γ2 Δ2 A B s :
   A === B ->
   Γ1 ⊢ B.[ren (+1)].[σ] : Sort s ->
   Γ2 ⊢ B : Sort s ->
   Γ1 ; Δ1 ⊢ σ ⊣ (A :: Γ2) ; (_: Δ2) ->
   Γ1 ; Δ1 ⊢ σ ⊣ (B :: Γ2) ; (_: Δ2)
-| dyn_agree_subst_conv1 Γ1 Δ1 σ Γ2 Δ2 A B s :
+| program_agree_subst_conv1 Γ1 Δ1 σ Γ2 Δ2 A B s :
   A === B ->
   Γ1 ⊢ B.[ren (+1)].[σ] : Sort s ->
   Γ2 ⊢ B : Sort s ->
   Γ1 ; Δ1 ⊢ σ ⊣ (A :: Γ2) ; (A :{s} Δ2) ->
   Γ1 ; Δ1 ⊢ σ ⊣ (B :: Γ2) ; (B :{s} Δ2)
-where "Γ1 ; Δ1 ⊢ σ ⊣ Γ2 ; Δ2" := (dyn_agree_subst Γ1 Δ1 σ Γ2 Δ2).
+where "Γ1 ; Δ1 ⊢ σ ⊣ Γ2 ; Δ2" := (program_agree_subst Γ1 Δ1 σ Γ2 Δ2).
 
-Lemma dyn_agree_subst_key Γ1 Γ2 Δ1 Δ2 σ s :
+Lemma program_agree_subst_key Γ1 Γ2 Δ1 Δ2 σ s :
   Γ1 ; Δ1 ⊢ σ ⊣ Γ2 ; Δ2 -> Δ2 ▷ s -> Δ1 ▷ s.
 Proof with eauto using key.
   move=>agr. elim: agr s=>{Γ1 Γ2 Δ1 Δ2 σ}...
@@ -56,14 +59,14 @@ Proof with eauto using key.
   { move=>Γ1 Δ1 σ Γ2 Δ2 A B s eq tyB1 tyB2 agr ih r k. inv k... }
 Qed.
 
-Lemma dyn_sta_agree_subst Γ1 Γ2 Δ1 Δ2 σ :
+Lemma program_logical_agree_subst Γ1 Γ2 Δ1 Δ2 σ :
   Γ1 ; Δ1 ⊢ σ ⊣ Γ2 ; Δ2 -> Γ1 ⊢ σ ⊣ Γ2.
-Proof with eauto using sta_agree_subst.
+Proof with eauto using logical_agree_subst.
   elim=>{Γ1 Γ2 Δ1 Δ2 σ}...
 Qed.
 
-Lemma dyn_agree_subst_refl Γ Δ : dyn_wf Γ Δ -> Γ ; Δ ⊢ ids ⊣ Γ ; Δ.
-Proof with eauto using dyn_agree_subst.
+Lemma program_agree_subst_refl Γ Δ : program_wf Γ Δ -> Γ ; Δ ⊢ ids ⊣ Γ ; Δ.
+Proof with eauto using program_agree_subst.
   elim: Γ Δ.
   { move=>Δ wf. inv wf... }
   { move=>A Γ ih Δ wf. inv wf.
@@ -74,36 +77,36 @@ Proof with eauto using dyn_agree_subst.
       have:(A.[ids] :: Γ); _: Δ0 ⊢ up ids ⊣ (A :: Γ); _: Δ0...
       by asimpl. } }
 Qed.
-#[global] Hint Resolve dyn_agree_subst_refl.
+#[global] Hint Resolve program_agree_subst_refl.
 
-Lemma dyn_agree_subst_has Γ1 Γ2 σ Δ1 Δ2 x s A :
-  Γ1 ; Δ1 ⊢ σ ⊣ Γ2 ; Δ2 -> dyn_wf Γ1 Δ1 -> dyn_has Δ2 x s A -> Γ1 ; Δ1 ⊢ (σ x) : A.[σ].
-Proof with eauto using dyn_agree_subst, dyn_agree_subst_key.
+Lemma program_agree_subst_has Γ1 Γ2 σ Δ1 Δ2 x s A :
+  Γ1 ; Δ1 ⊢ σ ⊣ Γ2 ; Δ2 -> program_wf Γ1 Δ1 -> program_has Δ2 x s A -> Γ1 ; Δ1 ⊢ (σ x) : A.[σ].
+Proof with eauto using program_agree_subst, program_agree_subst_key.
   move=>agr. elim: agr x s A=>{Γ1 Γ2 σ Δ1 Δ2}...
   { move=>σ x s A wf hs. inv hs. }
   { move=>Γ1 Δ1 σ Γ2 Δ2 A s agr ih tyA x t B wf hs.
     inv wf. inv hs; asimpl.
     replace A.[σ >> ren (+1)] with A.[σ].[ren (+1)] by autosubst.
-    apply: dyn_var; constructor...
+    apply: program_var; constructor...
     replace A0.[σ >> ren (+1)] with A0.[σ].[ren (+1)] by autosubst.
-    apply: dyn_eweakenU... }
+    apply: program_eweaken1... }
   { move=>Γ1 Δ1 σ Γ2 Δ2 A s agr ih tyA x t B wf hs.
     inv wf. inv hs; asimpl...
     replace A0.[σ >> ren (+1)] with A0.[σ].[ren (+1)]
       by autosubst.
-    apply: dyn_eweakenN... }
+    apply: program_eweaken0... }
   { move=>Γ1 Δ1 σ Γ2 Δ2 n A agr ih tyn x s B wf hs. inv hs; asimpl... }
   { move=>Γ1 Γ2 σ Δ1 Δ2 Δa Δb n A s k mrg agr ih tyn x t B wf hs.
     inv hs; asimpl.
-    { have ka:=dyn_agree_subst_key agr H5.
+    { have ka:=program_agree_subst_key agr H5.
       have->//:=merge_pureL mrg ka. }
     { have->:=merge_pureR mrg k.
       apply: ih...
-      have[]//:=dyn_wf_inv mrg wf. } }
+      have[]//:=program_wf_inv mrg wf. } }
   { move=>Γ1 Δ1 σ Γ2 Δ2 A B s eq tyB1 tyB2 agr ih x t C wf hs. inv hs.
-    { apply: dyn_conv.
-      apply: sta_conv_subst.
-      apply: sta_conv_subst...
+    { apply: program_conv.
+      apply: logical_conv_subst.
+      apply: logical_conv_subst...
       apply: ih...
       constructor...
       exact: tyB1. }
@@ -111,11 +114,11 @@ Proof with eauto using dyn_agree_subst, dyn_agree_subst_key.
       constructor... } }
 Qed.
 
-Lemma dyn_agree_subst_merge Γ1 Γ2 Δ1 Δ2 Δa Δb σ :
+Lemma program_agree_subst_merge Γ1 Γ2 Δ1 Δ2 Δa Δb σ :
   Γ1 ; Δ1 ⊢ σ ⊣ Γ2 ; Δ2 -> Δa ∘ Δb => Δ2 ->
   exists Δa' Δb',
     Δa' ∘ Δb' => Δ1 /\ Γ1 ; Δa' ⊢ σ ⊣ Γ2 ; Δa /\ Γ1 ; Δb' ⊢ σ ⊣ Γ2 ; Δb.
-Proof with eauto 6 using merge, dyn_agree_subst, dyn_agree_subst_key.
+Proof with eauto 6 using merge, program_agree_subst, program_agree_subst_key.
   move=>agr. elim: agr Δa Δb=>{Γ1 Γ2 Δ1 Δ2 σ}.
   { move=>σ Δa Δb mrg. inv mrg.
     exists nil. exists nil... }
@@ -137,7 +140,7 @@ Proof with eauto 6 using merge, dyn_agree_subst, dyn_agree_subst_key.
       have[Δc[mrg1 mrg2]]:=merge_splitL mrg mrg'.
       exists Δc. exists Δb'.
       repeat split...
-      apply: dyn_agree_subst_wk1...
+      apply: program_agree_subst_wk1...
       have[Δd[mrg3 mrg4]]:=merge_splitR mrg mrg'.
       have e:=merge_pureR mrg3 k.
       by subst. }
@@ -162,118 +165,119 @@ Proof with eauto 6 using merge, dyn_agree_subst, dyn_agree_subst_key.
       exists Δa'. exists Δb'... } }
 Qed.
 
-Lemma dyn_agree_subst_wf_nil Γ1 Δ1 σ : Γ1; Δ1 ⊢ σ ⊣ [::]; [::] → dyn_wf Γ1 Δ1.
-Proof with eauto using dyn_wf.
+Lemma program_agree_subst_wf_nil Γ1 Δ1 σ : Γ1; Δ1 ⊢ σ ⊣ [::]; [::] → program_wf Γ1 Δ1.
+Proof with eauto using program_wf.
   move e1:(nil)=>Γ2.
   move e2:(nil)=>Δ2 agr.
   elim: agr e1 e2=>//{Γ1 Γ2 Δ1 Δ2 σ}...
 Qed.
 
-Lemma dyn_agree_subst_wf_ty Γ1 Γ2 Δ1 Δ2 A s σ :
-  Γ1; Δ1 ⊢ σ ⊣ (A :: Γ2); A :{s} Δ2 -> dyn_wf Γ2 Δ2 ->
-  (∀ Γ1 Δ1 σ, Γ1; Δ1 ⊢ σ ⊣ Γ2; Δ2 → dyn_wf Γ1 Δ1) ->
-  dyn_wf Γ1 Δ1.
-Proof with eauto using dyn_wf.
+Lemma program_agree_subst_wf_ty Γ1 Γ2 Δ1 Δ2 A s σ :
+  Γ1; Δ1 ⊢ σ ⊣ (A :: Γ2); A :{s} Δ2 -> program_wf Γ2 Δ2 ->
+  (∀ Γ1 Δ1 σ, Γ1; Δ1 ⊢ σ ⊣ Γ2; Δ2 → program_wf Γ1 Δ1) ->
+  program_wf Γ1 Δ1.
+Proof with eauto using program_wf.
   move e1:(A :: Γ2)=>Γ0.
   move e2:(A :{s} Δ2)=>Δ0 agr.
   elim: agr A Γ2 Δ2 s e1 e2=>//{Γ0 Δ0 Γ1 Δ1 σ}...
   { move=>Γ1 Δ1 σ Γ2 Δ2 A s agr _ tyA A0 Γ0 Δ0 s0[e1 e2][_ e3 e4]wf h; subst.
-    apply: dyn_wf_ty...
+    apply: program_wf_ty...
     replace (Sort s) with (Sort s).[σ] by eauto.
-    apply: sta_substitution...
-    apply: dyn_sta_agree_subst... }
+    apply: logical_substitution...
+    apply: program_logical_agree_subst... }
   { move=>Γ1 Γ2 σ Δ1 Δ2 Δa Δb n A s k mrg agr _ tyn A0 Γ0 Δ0 s0
       [e1 e2][_ e3 e4]wf h; subst.
-    apply: dyn_wf_merge... }
+    apply: program_wf_merge... }
   { move=>Γ1 Δ1 σ Γ2 Δ2 A B s eq tyB1 tyB2 agr ih A0 Γ0 Δ0 s0
       [e1 e2][_ e3 e4]wf h; subst... }
 Qed.
 
-Lemma dyn_agree_subst_wf_n Γ1 Γ2 Δ1 Δ2 A σ :
-  Γ1; Δ1 ⊢ σ ⊣ (A :: Γ2); _: Δ2 -> dyn_wf Γ2 Δ2 ->
-  (∀ Γ1 Δ1 σ, Γ1; Δ1 ⊢ σ ⊣ Γ2; Δ2 → dyn_wf Γ1 Δ1) ->
-  dyn_wf Γ1 Δ1.
-Proof with eauto using dyn_wf.
+Lemma program_agree_subst_wf_n Γ1 Γ2 Δ1 Δ2 A σ :
+  Γ1; Δ1 ⊢ σ ⊣ (A :: Γ2); _: Δ2 -> program_wf Γ2 Δ2 ->
+  (∀ Γ1 Δ1 σ, Γ1; Δ1 ⊢ σ ⊣ Γ2; Δ2 → program_wf Γ1 Δ1) ->
+  program_wf Γ1 Δ1.
+Proof with eauto using program_wf.
   move e1:(A :: Γ2)=>Γ0.
   move e2:(_: Δ2)=>Δ0 agr.
   elim: agr A Γ2 Δ2 e1 e2=>//{Γ0 Δ0 Γ1 Δ1 σ}...
   { move=>Γ1 Δ1 σ Γ2 Δ2 A s agr _ tyA A0 Γ0 Δ0[e1 e2][e3]wf h; subst.
-    apply: dyn_wf_n...
-    have:=sta_substitution tyA (dyn_sta_agree_subst agr).
+    apply: program_wf_n...
+    have:=logical_substitution tyA (program_logical_agree_subst agr).
     asimpl... }
   { move=>Γ1 Δ1 σ Γ2 Δ2 n A agr ih tyn A0 Γ0 Δ0[e1 e2][e3]wf h; subst... }
   { move=>Γ1 Δ1 σ Γ2 Δ2 A B s eq tyB1 tyB2 agr ih A0 Γ0 Δ0
       [e1 e2][e3]wf h; subst... }
 Qed.
 
-Lemma dyn_substitution Γ1 Γ2 m A Δ1 Δ2 σ :
+(* Simultaneous substitution lemma. *)
+Lemma program_substitution Γ1 Γ2 m A Δ1 Δ2 σ :
   Γ2 ; Δ2 ⊢ m : A -> Γ1 ; Δ1 ⊢ σ ⊣ Γ2 ; Δ2 -> Γ1 ; Δ1 ⊢ m.[σ] : A.[σ].
-Proof with eauto using dyn_agree_subst, dyn_agree_subst_key, dyn_type.
+Proof with eauto using program_agree_subst, program_agree_subst_key, program_type.
   move=>ty. move:Γ2 Δ2 m A ty Γ1 Δ1 σ.
-  apply:(@dyn_type_mut _ (fun Γ2 Δ2 wf => forall Γ1 Δ1 σ, Γ1 ; Δ1 ⊢ σ ⊣ Γ2 ; Δ2 -> dyn_wf Γ1 Δ1)).
+  apply:(@program_type_mut _ (fun Γ2 Δ2 wf => forall Γ1 Δ1 σ, Γ1 ; Δ1 ⊢ σ ⊣ Γ2 ; Δ2 -> program_wf Γ1 Δ1)).
   { move=>Γ Δ x s A wf h shs dhs Γ1 Δ1 σ agr. asimpl.
-    apply: dyn_agree_subst_has... }
+    apply: program_agree_subst_has... }
   { move=>Γ Δ A B m s k tym ihm Γ1 Δ1 σ agr. asimpl.
-    have wf:=dyn_type_wf tym. inv wf.
-    apply: dyn_lam0... }
+    have wf:=program_type_wf tym. inv wf.
+    apply: program_lam0... }
   { move=>Γ Δ A B m s t k tym ihm Γ1 Δ1 σ agr. asimpl.
-    have wf:=dyn_type_wf tym. inv wf.
-    apply: dyn_lam1... }
+    have wf:=program_type_wf tym. inv wf.
+    apply: program_lam1... }
   { move=>Γ Δ A B m n s tym ihm tyn Γ1 Δ1 σ agr. asimpl.
     replace B.[n.[σ] .: σ] with B.[up σ].[n.[σ]/] by autosubst.
     have{}ihm:=ihm _ _ _ agr.
-    apply: dyn_app0...
-    have//:=sta_substitution tyn (dyn_sta_agree_subst agr). }
+    apply: program_app0...
+    have//:=logical_substitution tyn (program_logical_agree_subst agr). }
   { move=>Γ Δ1 Δ2 Δ A B m n s mrg tym ihm tyn ihn Γ1 Δ0 σ agr. asimpl.
     replace B.[n.[σ] .: σ] with B.[up σ].[n.[σ]/] by autosubst.
-    have[Δa[Δb[mrg0[agra agrb]]]]:=dyn_agree_subst_merge agr mrg.
+    have[Δa[Δb[mrg0[agra agrb]]]]:=program_agree_subst_merge agr mrg.
     have{}ihm:=ihm _ _ _ agra.
     have{}ihn:=ihn _ _ _ agrb.
-    apply: dyn_app1... }
+    apply: program_app1... }
   { move=>Γ Δ A B m n t tyS tym ihm tyn Γ1 Δ1 σ agr. asimpl.
-    have{}ihS:=sta_substitution tyS (dyn_sta_agree_subst agr).
+    have{}ihS:=logical_substitution tyS (program_logical_agree_subst agr).
     have{}ihm:=ihm _ _ _ agr.
-    have{}ihn:=sta_substitution tyn (dyn_sta_agree_subst agr).
-    apply: dyn_pair0...
+    have{}ihn:=logical_substitution tyn (program_logical_agree_subst agr).
+    apply: program_pair0...
     asimpl. asimpl in ihn... }
   { move=>Γ Δ1 Δ2 Δ A B m n t mrg tyS tym ihm tyn ihn Γ1 Δ0 σ agr. asimpl.
-    have[Δa[Δb[mrg0[agra agrb]]]]:=dyn_agree_subst_merge agr mrg.
-    have{}ihS:=sta_substitution tyS (dyn_sta_agree_subst agr).
+    have[Δa[Δb[mrg0[agra agrb]]]]:=program_agree_subst_merge agr mrg.
+    have{}ihS:=logical_substitution tyS (program_logical_agree_subst agr).
     have{}ihm:=ihm _ _ _ agra.
     have{}ihn:=ihn _ _ _ agrb.
-    apply: dyn_pair1...
+    apply: program_pair1...
     asimpl. asimpl in ihn... }
   { move=>Γ Δ1 Δ2 Δ A B C m n s r t mrg tyC tym ihm tyn ihn Γ1 Δ0 σ agr. asimpl.
-    have[Δa[Δb[mrg0[agra agrb]]]]:=dyn_agree_subst_merge agr mrg.
+    have[Δa[Δb[mrg0[agra agrb]]]]:=program_agree_subst_merge agr mrg.
     replace C.[m.[σ] .: σ] with C.[up σ].[m.[σ]/] by autosubst.
-    have wf:=sta_type_wf tyC. inv wf.
-    have wf:=dyn_type_wf tyn. inv wf. inv H4.
-    have{}ihC:=sta_substitution tyC (sta_agree_subst_ty (dyn_sta_agree_subst agr) H2).
+    have wf:=logical_type_wf tyC. inv wf.
+    have wf:=program_type_wf tyn. inv wf. inv H4.
+    have{}ihC:=logical_substitution tyC (logical_agree_subst_ty (program_logical_agree_subst agr) H2).
     have{}ihm:=ihm _ _ _ agra.
-    have{}ihn:=ihn _ _ _ (dyn_agree_subst_n (dyn_agree_subst_ty agrb H8) H5).
-    apply: dyn_letin0...
+    have{}ihn:=ihn _ _ _ (program_agree_subst_n (program_agree_subst_ty agrb H8) H5).
+    apply: program_letin0...
     asimpl. asimpl in ihn... }
   { move=>Γ Δ1 Δ2 Δ A B C m n s r1 r2 t mrg tyC tym ihm tyn ihn Γ1 Δ0 σ agr. asimpl.
-    have[Δa[Δb[mrg0[agra agrb]]]]:=dyn_agree_subst_merge agr mrg.
+    have[Δa[Δb[mrg0[agra agrb]]]]:=program_agree_subst_merge agr mrg.
     replace C.[m.[σ] .: σ] with C.[up σ].[m.[σ]/] by autosubst.
-    have wf:=sta_type_wf tyC. inv wf.
-    have wf:=dyn_type_wf tyn. inv wf. inv H4.
-    have{}ihC:=sta_substitution tyC (sta_agree_subst_ty (dyn_sta_agree_subst agr) H2).
+    have wf:=logical_type_wf tyC. inv wf.
+    have wf:=program_type_wf tyn. inv wf. inv H4.
+    have{}ihC:=logical_substitution tyC (logical_agree_subst_ty (program_logical_agree_subst agr) H2).
     have{}ihm:=ihm _ _ _ agra.
-    have{}ihn:=ihn _ _ _ (dyn_agree_subst_ty (dyn_agree_subst_ty agrb H8) H6).
-    apply: dyn_letin1...
+    have{}ihn:=ihn _ _ _ (program_agree_subst_ty (program_agree_subst_ty agrb H8) H6).
+    apply: program_letin1...
     asimpl. asimpl in ihn... }
-  { move=>Γ Δ A B m n t k tym ihm tyn ihn Γ1 Δ1 σ agr. asimpl. apply: dyn_apair... }
-  { move=>Γ Δ A B m t tym ihm Γ1 Δ1 σ agr. asimpl. apply: dyn_fst... }
-  { move=>Γ Δ A B m t tym ihm Γ1 Δ1 σ agr. asimpl. apply: dyn_snd... }
+  { move=>Γ Δ A B m n t k tym ihm tyn ihn Γ1 Δ1 σ agr. asimpl. apply: program_apair... }
+  { move=>Γ Δ A B m t tym ihm Γ1 Δ1 σ agr. asimpl. apply: program_fst... }
+  { move=>Γ Δ A B m t tym ihm Γ1 Δ1 σ agr. asimpl. apply: program_snd... }
   { move=>Γ Δ A B H P m n s tyB tyH ihH tyP Γ1 Δ1 σ agr. asimpl.
     replace B.[P.[σ] .: n.[σ] .: σ] with B.[upn 2 σ].[P.[σ],n.[σ]/] by autosubst.
-    have wf:=sta_type_wf tyB. inv wf. inv H2.
-    have agr':=dyn_sta_agree_subst agr.
-    have ihB:=sta_substitution tyB (sta_agree_subst_ty (sta_agree_subst_ty agr' H5) H3).
-    have ihP:=sta_substitution tyP agr'.
+    have wf:=logical_type_wf tyB. inv wf. inv H2.
+    have agr':=program_logical_agree_subst agr.
+    have ihB:=logical_substitution tyB (logical_agree_subst_ty (logical_agree_subst_ty agr' H5) H3).
+    have ihP:=logical_substitution tyP agr'.
     have{}ihH:=ihH _ _ _ agr.
-    apply: dyn_rw.
+    apply: program_rw.
     asimpl in ihB.
     replace A.[σ >> ren (+1)] with A.[σ].[ren (+1)] in ihB by autosubst.
     replace m.[σ >> ren (+1)] with m.[σ].[ren (+1)] in ihB by autosubst.
@@ -281,90 +285,96 @@ Proof with eauto using dyn_agree_subst, dyn_agree_subst_key, dyn_type.
     asimpl. asimpl in ihH...
     asimpl in ihP... }
   { move=>Γ Δ A B m s eq tym ihm tyB Γ1 Δ1 σ agr.
-    apply: dyn_conv.
-    apply: sta_conv_subst...
+    apply: program_conv.
+    apply: logical_conv_subst...
     apply: ihm...
-    have:=sta_substitution tyB (dyn_sta_agree_subst agr).
+    have:=logical_substitution tyB (program_logical_agree_subst agr).
     asimpl... }
-  { exact: dyn_agree_subst_wf_nil. }
+  { exact: program_agree_subst_wf_nil. }
   { move=>Γ Δ A s wf h tyA Γ1 Δ1 σ agr.
-    apply: dyn_agree_subst_wf_ty... }
+    apply: program_agree_subst_wf_ty... }
   { move=>Γ Δ A s wf ih tyA Γ1 Δ1 σ agr.
-    apply: dyn_agree_subst_wf_n... }
+    apply: program_agree_subst_wf_n... }
 Qed.
 
-Lemma dyn_substitution_wf Γ1 Γ2 Δ1 Δ2 σ :
-  dyn_wf Γ2 Δ2 -> Γ1 ; Δ1 ⊢ σ ⊣ Γ2 ; Δ2 -> dyn_wf Γ1 Δ1.
-Proof with eauto using dyn_wf.
+Lemma program_substitution_wf Γ1 Γ2 Δ1 Δ2 σ :
+  program_wf Γ2 Δ2 -> Γ1 ; Δ1 ⊢ σ ⊣ Γ2 ; Δ2 -> program_wf Γ1 Δ1.
+Proof with eauto using program_wf.
   move=>wf. elim: wf Γ1 Δ1 σ=>{Γ2 Δ2}.
-  { move=>*. apply: dyn_agree_subst_wf_nil... }
-  { move=>*. apply: dyn_agree_subst_wf_ty... }
-  { move=>*. apply: dyn_agree_subst_wf_n... }
+  { move=>*. apply: program_agree_subst_wf_nil... }
+  { move=>*. apply: program_agree_subst_wf_ty... }
+  { move=>*. apply: program_agree_subst_wf_n... }
 Qed.
 
-Lemma dyn_subst0 Γ Δ m n A B :
+(* Lemma 5 (Program 0-Substitution) *)
+Lemma program_subst0 Γ Δ m n A B :
   (A :: Γ) ; _: Δ ⊢ m : B -> Γ ⊢ n : A -> Γ ; Δ ⊢ m.[n/] : B.[n/].
-Proof with eauto using dyn_agree_subst_refl.
+Proof with eauto using program_agree_subst_refl.
   move=>tym tyn.
-  have wf:=dyn_type_wf tym. inv wf.
-  apply: dyn_substitution...
-  apply: dyn_agree_subst_wk0...
+  have wf:=program_type_wf tym. inv wf.
+  apply: program_substitution...
+  apply: program_agree_subst_wk0...
   by asimpl.
 Qed.
 
-Lemma dyn_subst1 Γ Δ1 Δ2 Δ m n A B s :
+(* Lemma 6 (Program 1-Substitution) *)
+Lemma program_subst1 Γ Δ1 Δ2 Δ m n A B s :
   Δ2 ▷ s -> Δ1 ∘ Δ2 => Δ ->
   (A :: Γ) ; A :{s} Δ1 ⊢ m : B -> Γ ; Δ2 ⊢ n : A -> Γ ; Δ ⊢ m.[n/] : B.[n/].
-Proof with eauto using dyn_agree_subst_refl.
+Proof with eauto using program_agree_subst_refl.
   move=>k mrg tym tyn.
-  have wf:=dyn_type_wf tym. inv wf.
-  apply: dyn_substitution...
-  apply: dyn_agree_subst_wk1...
+  have wf:=program_type_wf tym. inv wf.
+  apply: program_substitution...
+  apply: program_agree_subst_wk1...
   by asimpl.
 Qed.
 
-Lemma dyn_esubst0 Γ Δ m m' n A B B' :
+(* Alternative statement more suitable for certain Coq tactics *)
+Lemma program_esubst0 Γ Δ m m' n A B B' :
   m' = m.[n/] ->
   B' = B.[n/] ->
   (A :: Γ) ; _: Δ ⊢ m : B -> Γ ⊢ n : A -> Γ ; Δ ⊢ m': B'.
 Proof.
-  move=>*; subst. apply: dyn_subst0; eauto.
+  move=>*; subst. apply: program_subst0; eauto.
 Qed.
 
-Lemma dyn_esubst1 Γ Δ1 Δ2 Δ m m' n A B B' s :
+(* Alternative statement more suitable for certain Coq tactics *)
+Lemma program_esubst1 Γ Δ1 Δ2 Δ m m' n A B B' s :
   m' = m.[n/] ->
   B' = B.[n/] ->
   Δ2 ▷ s -> Δ1 ∘ Δ2 => Δ ->
   (A :: Γ) ; A :{s} Δ1 ⊢ m : B -> Γ ; Δ2 ⊢ n : A -> Γ ; Δ ⊢ m' : B'.
 Proof.
-  move=>*; subst. apply: dyn_subst1; eauto.
+  move=>*; subst. apply: program_subst1; eauto.
 Qed.
 
-Lemma dyn_ctx_conv0 Γ Δ m A B C s :
+(* Context conversion lemma for the logical context. *)
+Lemma program_ctx_conv0 Γ Δ m A B C s :
   B === A ->
   Γ ⊢ B : Sort s -> (A :: Γ) ; _: Δ ⊢ m : C -> (B :: Γ) ; _: Δ ⊢ m : C.
-Proof with eauto using dyn_wf, dyn_agree_subst_refl.
+Proof with eauto using program_wf, program_agree_subst_refl.
   move=>eq tyB tym.
-  have wf:=dyn_type_wf tym. inv wf.
+  have wf:=program_type_wf tym. inv wf.
   have:(B :: Γ) ; _: Δ ⊢ m.[ids] : C.[ids].
-  apply: dyn_substitution...
-  apply: dyn_agree_subst_conv0...
-  apply: sta_eweaken...
+  apply: program_substitution...
+  apply: program_agree_subst_conv0...
+  apply: logical_eweaken...
   asimpl...
   asimpl...
   asimpl...
 Qed.
 
-Lemma dyn_ctx_conv1 Γ Δ m A B C s :
+(* Context conversion lemma for the program context. *)
+Lemma program_ctx_conv1 Γ Δ m A B C s :
   B === A ->
   Γ ⊢ B : Sort s -> (A :: Γ) ; A :{s} Δ ⊢ m : C -> (B :: Γ) ; B :{s} Δ ⊢ m : C.
-Proof with eauto using dyn_wf, dyn_agree_subst_refl.
+Proof with eauto using program_wf, program_agree_subst_refl.
   move=>eq tyB tym.
-  have wf:=dyn_type_wf tym. inv wf.
+  have wf:=program_type_wf tym. inv wf.
   have:(B :: Γ) ; B :{s} Δ ⊢ m.[ids] : C.[ids].
-  apply: dyn_substitution...
-  apply: dyn_agree_subst_conv1...
-  apply: sta_eweaken...
+  apply: program_substitution...
+  apply: program_agree_subst_conv1...
+  apply: logical_eweaken...
   asimpl...
   asimpl...
   asimpl...
