coq/theories/erasure_sr.v
@@ -1,14 +1,17 @@
+(* This file presents the erasure subject reduction theorem. *)
+
 From mathcomp Require Import ssreflect ssrbool eqtype ssrnat seq.
 From Coq Require Import ssrfun Classical Utf8.
-Require Export AutosubstSsr ARS dyn_prog era_inv.
+Require Export AutosubstSsr ARS program_prog erasure_inv.
 
 Set Implicit Arguments.
 Unset Strict Implicit.
 Unset Printing Implicit Defensive.
 
-Lemma era_dyn_val Γ Δ m m' A :
-  Γ ; Δ ⊢ m ~ m' : A -> dyn_val m' -> dyn_val m.
-Proof with eauto using dyn_val.
+(* The preimage of values under erasure are values. *)
+Lemma erasure_program_val Γ Δ m m' A :
+  Γ ; Δ ⊢ m ~ m' : A -> program_val m' -> program_val m.
+Proof with eauto using program_val.
   move=>ty. elim: ty=>{Γ Δ m m' A}...
   { move=>Γ Δ A B m m' n s tym ihm tyn vl. inv vl. }
   { move=>Γ Δ1 Δ2 Δ A B m m' n n' s mrg tym ihm tyn ihn vl. inv vl. }
@@ -21,10 +24,11 @@ Proof with eauto using dyn_val.
   { move=>Γ Δ A B H H' P m n s tyB tyH ihH tyP vl. inv vl. }
 Qed.
 
-Theorem era_sr m m' n' A :
+(* Theorem 11 (Erasure Subject Reduction)  *)
+Theorem erasure_sr m m' n' A :
   nil ; nil ⊢ m ~ m' : A -> m' ~>> n' ->
   exists2 n, m ~>> n & nil ; nil ⊢ n ~ n' : A.
-Proof with eauto using dyn_step, era_type, dyn_val, merge.
+Proof with eauto using program_step, erasure_type, program_val, merge.
   move e1:(nil)=>Γ.
   move e2:(nil)=>Δ er. elim: er e1 e2 n'=>{Γ Δ m m' A}.
   { move=>Γ Δ x s A wf shs dhs e1 e2 n' st. inv st. }
@@ -33,171 +37,172 @@ Proof with eauto using dyn_step, era_type, dyn_val, merge.
   { move=>Γ Δ A B m m' n s erm ihm tyn e1 e2 n' st. inv st.
     { have[x st tyx]:=ihm erefl erefl _ H2. exists (App x n)... }
     { inv H2. }
-    { have[A'[m' e]]:=era_lam0_form erm.
+    { have[A'[m' e]]:=erasure_lam0_form erm.
       subst. exists (m'.[n/])...
-      apply: era_subst0...
-      have[//]:=era_lam0_inv erm. }
-    { have[A'[m' e]]:=era_lam1_form erm. subst.
-      have/dyn_sta_type ty:=era_dyn_type erm.
-      exfalso. apply: sta_lam1_pi0_false... } }
+      apply: erasure_subst0...
+      have[//]:=erasure_lam0_inv erm. }
+    { have[A'[m' e]]:=erasure_lam1_form erm. subst.
+      have/program_logical_reflect ty:=erasure_program_reflect erm.
+      exfalso. apply: logical_lam1_pi0_false... } }
   { move=>Γ Δ1 Δ2 Δ A B m m' n n' s mrg erm ihm ern ihn e1 e2 x st.
     subst. inv mrg. inv st.
     { have[x st tyx]:=ihm erefl erefl _ H2. exists (App x n)... }
     { have[x st tyx]:=ihn erefl erefl _ H2. exists (App m x)...
-      have tym:=era_dyn_type erm.
-      have/dyn_sta_type tyn:=era_dyn_type ern.
-      have[_/sta_pi1_inv[r[tyB _]]]:=dyn_valid tym.
-      apply: era_conv.
-      apply: sta_conv_beta.
+      have tym:=erasure_program_reflect erm.
+      have/program_logical_reflect tyn:=erasure_program_reflect ern.
+      have[_/logical_pi1_inv[r[tyB _]]]:=program_valid tym.
+      apply: erasure_conv.
+      apply: logical_conv_beta.
       apply: conv_sym.
       apply: star_conv.
-      apply: dyn_sta_step...
-      apply: era_app1...
-      have:=sta_subst tyB tyn.
+      apply: program_logical_step...
+      apply: erasure_app1...
+      have:=logical_subst tyB tyn.
       asimpl... }
-    { have[A'[m' e]]:=era_lam0_form erm. subst.
-      have/dyn_sta_type ty:=era_dyn_type erm.
-      exfalso. apply: sta_lam0_pi1_false... }
-    { have[A'[m' e]]:=era_lam1_form erm.
+    { have[A'[m' e]]:=erasure_lam0_form erm. subst.
+      have/program_logical_reflect ty:=erasure_program_reflect erm.
+      exfalso. apply: logical_lam0_pi1_false... }
+    { have[A'[m' e]]:=erasure_lam1_form erm.
       subst. exists (m'.[n/])...
-      apply: dyn_step_beta1.
-      apply: era_dyn_val...
-      have{erm}[t[erm _]]:=era_lam1_inv erm.
-      have wf:=dyn_type_wf (era_dyn_type erm). inv wf.
-      apply: era_subst1...
-      apply: dyn_val_key.
-      apply: (era_dyn_type ern)...
+      apply: program_step_beta1.
+      apply: erasure_program_val...
+      have{erm}[t[erm _]]:=erasure_lam1_inv erm.
+      have wf:=program_type_wf (erasure_program_reflect erm). inv wf.
+      apply: erasure_subst1...
+      apply: program_val_stability.
+      apply: (erasure_program_reflect ern)...
       exact: H5.
-      apply: era_dyn_val... } }
+      apply: erasure_program_val... } }
   { move=>Γ Δ A B m m' n t tyS erm ihm tyn e1 e2 x st. inv st.
-    have[s[r[ord[tyA[tyB _]]]]]:=sta_sig0_inv tyS.
+    have[s[r[ord[tyA[tyB _]]]]]:=logical_sig0_inv tyS.
     have[x st erx]:=ihm erefl erefl _ H3. exists (Pair0 x n t)...
-    apply: era_pair0...
-    apply: sta_conv.
-    apply: sta_conv_beta.
+    apply: erasure_pair0...
+    apply: logical_conv.
+    apply: logical_conv_beta.
     apply: star_conv.
-    apply: (dyn_sta_step (dyn_sta_type (era_dyn_type erm)))...
+    apply: (program_logical_step (program_logical_reflect (erasure_program_reflect erm)))...
     apply: tyn.
-    apply: sta_esubst...
+    apply: logical_esubst...
     by autosubst. }
   { move=>Γ Δ1 Δ2 Δ A B m m' n n' t mrg tyS erm ihm ern ihn e1 e2 x st.
-    have[s[r[ord1[ord2[tyA[tyB _]]]]]]:=sta_sig1_inv tyS.
+    have[s[r[ord1[ord2[tyA[tyB _]]]]]]:=logical_sig1_inv tyS.
     subst. inv mrg. inv st.
     { have[x st erx]:=ihm erefl erefl _ H3. exists (Pair1 x n t)...
-      apply: era_pair1...
-      apply: era_conv.
-      apply: sta_conv_beta.
+      apply: erasure_pair1...
+      apply: erasure_conv.
+      apply: logical_conv_beta.
       apply: star_conv.
-      apply: (dyn_sta_step (dyn_sta_type (era_dyn_type erm)))...
+      apply: (program_logical_step (program_logical_reflect (erasure_program_reflect erm)))...
       apply: ern.
-      apply: sta_esubst...
+      apply: logical_esubst...
       by autosubst. }
     { have[x st erx]:=ihn erefl erefl _ H3. exists (Pair1 m x t)... } }
   { move=>Γ Δ1 Δ2 Δ A B C m m' n n' s r t mrg tyC erm ihm ern ihn e1 e2 x st.
     subst. inv mrg. inv st.
     { have[x st erx]:=ihm erefl erefl _ H3. exists (LetIn C x n)...
-      apply: era_conv.
-      apply: sta_conv_beta.
+      apply: erasure_conv.
+      apply: logical_conv_beta.
       apply: conv_sym.
       apply: star_conv.
-      apply: (dyn_sta_step (dyn_sta_type (era_dyn_type erm)))...
-      apply: era_letin0...
-      apply: sta_esubst...
+      apply: (program_logical_step (program_logical_reflect (erasure_program_reflect erm)))...
+      apply: erasure_letin0...
+      apply: logical_esubst...
       by autosubst. }
-    { have[m3[m4 e]]:=era_pair0_form erm. subst.
-      have wf:=dyn_type_wf (era_dyn_type ern). inv wf. inv H2.
-      have[e1[e2[erm3 tym4]]]:=era_pair0_inv erm. subst.
-      have vl:dyn_val (Pair0 m3 m4 t) by (apply: era_dyn_val; eauto).
+    { have[m3[m4 e]]:=erasure_pair0_form erm. subst.
+      have wf:=program_type_wf (erasure_program_reflect ern). inv wf. inv H2.
+      have[e1[e2[erm3 tym4]]]:=erasure_pair0_inv erm. subst.
+      have vl:program_val (Pair0 m3 m4 t) by (apply: erasure_program_val; eauto).
       exists (n.[m4,m3/])...
       replace C.[Pair0 m3 m4 t/]
         with C.[Pair0 (Var 1) (Var 0) t .: ren (+2)].[m4,m3/] by autosubst.
-      apply: era_substitution...
-      apply: era_agree_subst_wk0...
-      apply: era_agree_subst_wk1.
-      apply: (dyn_val_key (era_dyn_type erm3) H7).
+      apply: erasure_substitution...
+      apply: erasure_agree_subst_wk0...
+      apply: erasure_agree_subst_wk1.
+      apply: (program_val_stability (erasure_program_reflect erm3) H7).
       inv vl...
       apply: merge_sym...
-      apply: era_agree_subst_refl...
+      apply: erasure_agree_subst_refl...
       by autosubst. }
-    { have[m3[m4 e]]:=era_pair1_form erm. subst.
-      have/dyn_sta_type ty:=era_dyn_type erm.
-      exfalso. apply: sta_pair1_sig0_false... } }
+    { have[m3[m4 e]]:=erasure_pair1_form erm. subst.
+      have/program_logical_reflect ty:=erasure_program_reflect erm.
+      exfalso. apply: logical_pair1_sig0_false... } }
   { move=>Γ Δ1 Δ2 Δ A B C m m' n n' s r1 r2 t mrg tyC erm ihm ern ihn e1 e2 x st.
     subst. inv mrg. inv st.
     { have[x st erx]:=ihm erefl erefl _ H3. exists (LetIn C x n)...
-      apply: era_conv.
-      apply: sta_conv_beta.
+      apply: erasure_conv.
+      apply: logical_conv_beta.
       apply: conv_sym.
       apply: star_conv.
-      apply: (dyn_sta_step (dyn_sta_type (era_dyn_type erm)))...
-      apply: era_letin1...
-      apply: sta_esubst...
+      apply: (program_logical_step (program_logical_reflect (erasure_program_reflect erm)))...
+      apply: erasure_letin1...
+      apply: logical_esubst...
       by autosubst. }
-    { have[m3[m4 e]]:=era_pair0_form erm. subst.
-      have/dyn_sta_type ty:=era_dyn_type erm.
-      exfalso. apply: sta_pair0_sig1_false... }
-    { have[m3[m4 e]]:=era_pair1_form erm. subst.
-      have wf:=dyn_type_wf (era_dyn_type ern). inv wf. inv H2.
-      have[Δ1'[Δ2'[mrg'[e[erm3 erm4]]]]]:=era_pair1_inv erm.
+    { have[m3[m4 e]]:=erasure_pair0_form erm. subst.
+      have/program_logical_reflect ty:=erasure_program_reflect erm.
+      exfalso. apply: logical_pair0_sig1_false... }
+    { have[m3[m4 e]]:=erasure_pair1_form erm. subst.
+      have wf:=program_type_wf (erasure_program_reflect ern). inv wf. inv H2.
+      have[Δ1'[Δ2'[mrg'[e[erm3 erm4]]]]]:=erasure_pair1_inv erm.
       subst. inv mrg'.
-      have tym3:=era_dyn_type erm3.
-      have tym4:=era_dyn_type erm4.
-      have vl:dyn_val (Pair1 m3 m4 t) by (apply: era_dyn_val; eauto). inv vl.
-      have k1:=dyn_val_key tym3 H7 H1.
-      have k2:=dyn_val_key tym4 (sta_subst H5 (dyn_sta_type tym3)) H6.
+      have tym3:=erasure_program_reflect erm3.
+      have tym4:=erasure_program_reflect erm4.
+      have vl:program_val (Pair1 m3 m4 t) by (apply: erasure_program_val; eauto). inv vl.
+      have k1:=program_val_stability tym3 H7 H1.
+      have k2:=program_val_stability tym4 (logical_subst H5 (program_logical_reflect tym3)) H6.
       exists (n.[m4,m3/])...
       replace C.[Pair1 m3 m4 t/]
         with C.[Pair1 (Var 1) (Var 0) t .: ren (+2)].[m4,m3/] by autosubst.
-      apply: era_substitution...
-      apply: era_agree_subst_wk1...
-      apply: era_agree_subst_wk1...
+      apply: erasure_substitution...
+      apply: erasure_agree_subst_wk1...
+      apply: erasure_agree_subst_wk1...
       by autosubst. } }
   { move=>Γ Δ A B m m' n n' t k erm ihm tyn ihn e1 e2 x st. inv st. }
   { move=>Γ Δ A B m m' t tym ihm e1 e2 x st. inv st.
     { have[x st erx]:=ihm erefl erefl _ H0. exists (Fst x)... }
-    { have[m1[m2 e]]:=era_apair_form tym. subst.
-      have[e[erm1 erm2]]:=era_apair_inv tym.
+    { have[m1[m2 e]]:=erasure_apair_form tym. subst.
+      have[e[erm1 erm2]]:=erasure_apair_inv tym.
       subst. exists m1... } }
   { move=>Γ Δ A B m m' t tym ihm e1 e2 x st. inv st.
     { have[x st erx]:=ihm erefl erefl _ H0. exists (Snd x)... }
-    { have[m1[m2 e]]:=era_apair_form tym. subst.
-      have[e[erm1 erm2]]:=era_apair_inv tym.
+    { have[m1[m2 e]]:=erasure_apair_form tym. subst.
+      have[e[erm1 erm2]]:=erasure_apair_inv tym.
       subst. exists m2... } }
   { move=>Γ Δ A B H H' P m n s tyB erH ihH tyP e1 e2 x st. inv st.
-    have[P0[rdP vlP]]:=sta_vn tyP.
-    have tyP0:=sta_rd tyP rdP.
-    have[n0 e]:=sta_id_canonical tyP0 (convR _ _) vlP. subst.
-    have tyr:=sta_rd tyP rdP.
-    have[r tyI]:=sta_valid tyP.
-    have[tym[tyn/sort_inj e]]:=sta_id_inv tyI. subst.
-    have[tym0[eq1 eq2]]:=sta_refl_inv tyr.
+    have[P0[rdP vlP]]:=logical_vn tyP.
+    have tyP0:=logical_rd tyP rdP.
+    have[n0 e]:=logical_id_canonical tyP0 (convR _ _) vlP. subst.
+    have tyr:=logical_rd tyP rdP.
+    have[r tyI]:=logical_valid tyP.
+    have[tym[tyn/sort_inj e]]:=logical_id_inv tyI. subst.
+    have[tym0[eq1 eq2]]:=logical_refl_inv tyr.
     have sc:sconv (Refl m .: m .: ids) (P .: n .: ids).
     { move=>[|[|]]//=.
-      apply: conv_trans. apply: sta_conv_refl. apply: conv_sym...
+      apply: conv_trans. apply: logical_conv_refl. apply: conv_sym...
       apply: conv_sym. apply: star_conv...
       apply: conv_trans. apply: conv_sym... eauto. }
     have wkB:nil ⊢ B.[P,n/] : Sort s.
     { replace (Sort s) with (Sort s).[P,n/] by eauto.
-      apply: sta_substitution...
+      apply: logical_substitution...
       repeat constructor...
       all: asimpl... }
     exists H...
-    apply: era_conv.
-    apply: sta_conv_compat sc.
+    apply: erasure_conv.
+    apply: logical_conv_compat sc.
     all: eauto. }
   { move=>Γ Δ A B m m' s eq tym ihm tyB e1 e2 n' st. subst.
     have[n st' tyn]:=ihm erefl erefl _ st.
     exists n... }
 Qed.
 
-Corollary era_rd m m' n' A :
+(* Iterated steps preserve the erasure relation. *)
+Corollary erasure_rd m m' n' A :
   nil ; nil ⊢ m ~ m' : A -> m' ~>>* n' ->
   exists2 n, m ~>>* n & nil ; nil ⊢ n ~ n' : A.
 Proof with eauto.
   move=>ty rd. elim: rd m A ty=>{n'}...
   move=>n n' rd ih st m A tym.
   have[x rdx tyx]:=ih _ _ tym.
-  have[y sty tyy]:=era_sr tyx st.
+  have[y sty tyy]:=erasure_sr tyx st.
   exists y...
   apply: star_trans...
   apply: star1...
