coq/theories/erasure_weak.v
@@ -1,146 +1,142 @@
+(* This file presents the program weakening lemmas instrumented
+   to cover the erasure procedure. *)
+
 From mathcomp Require Import ssreflect ssrbool eqtype ssrnat seq.
 From Coq Require Import ssrfun Classical Utf8.
-Require Export AutosubstSsr ARS era_type.
+Require Export AutosubstSsr ARS erasure_type.
 
 Set Implicit Arguments.
 Unset Strict Implicit.
 Unset Printing Implicit Defensive.
 
-Lemma era_rename Γ Γ' Δ Δ' m m' A ξ :
-  Γ ; Δ ⊢ m ~ m' : A -> dyn_agree_ren ξ Γ Δ Γ' Δ' ->
+(* Generalized renaming lemma. *)
+Lemma erasure_rename Γ Γ' Δ Δ' m m' A ξ :
+  Γ ; Δ ⊢ m ~ m' : A -> program_agree_ren ξ Γ Δ Γ' Δ' ->
   Γ' ; Δ' ⊢ m.[ren ξ] ~ m'.[ren ξ] : A.[ren ξ].
 Proof with eauto using
-  era_type, sta_agree_ren, dyn_agree_ren, dyn_agree_ren_key.
+  erasure_type, logical_agree_ren, program_agree_ren, program_agree_ren_key.
   move=>ty. elim: ty Γ' Δ' ξ=>{Γ Δ m m' A}.
   { move=>Γ Δ x s A wf shs dhs Γ' Δ' ξ agr. asimpl.
-    apply: era_var.
-    apply: dyn_rename_wf...
-    apply: sta_agree_ren_has...
-    apply: dyn_sta_agree_ren...
-    apply: dyn_agree_ren_has... }
+    apply: erasure_var.
+    apply: program_rename_wf...
+    apply: logical_agree_ren_has...
+    apply: program_logical_agree_ren...
+    apply: program_agree_ren_has... }
   { move=>Γ Δ A B m m' s k tym ihm Γ' Δ' ξ agr. asimpl.
-    have wf:=dyn_type_wf (era_dyn_type tym). inv wf.
-    apply: era_lam0... }
+    have wf:=program_type_wf (erasure_program_reflect tym). inv wf.
+    apply: erasure_lam0... }
   { move=>Γ Δ A B m m' s t k tym ihm Γ' Δ' ξ agr. asimpl.
-    have wf:=dyn_type_wf (era_dyn_type tym). inv wf.
-    apply: era_lam1... }
+    have wf:=program_type_wf (erasure_program_reflect tym). inv wf.
+    apply: erasure_lam1... }
   { move=>Γ Δ A B m m' n s tym ihm tyn Γ' Δ' ξ agr. asimpl.
     replace B.[n.[ren ξ] .: ren ξ] with B.[ren (upren ξ)].[n.[ren ξ]/]
       by autosubst.
     have{}ihm:=ihm _ _ _ agr.
-    have{}ihn:=sta_rename tyn (dyn_sta_agree_ren agr).
-    apply: era_app0...
+    have{}ihn:=logical_rename tyn (program_logical_agree_ren agr).
+    apply: erasure_app0...
     asimpl in ihm... }
   { move=>Γ Δ1 Δ2 Δ A B m m' n n' s mrg tym ihm tyn ihn Γ' Δ' ξ agr. asimpl.
     replace B.[n.[ren ξ] .: ren ξ] with B.[ren (upren ξ)].[n.[ren ξ]/]
       by autosubst.
-    have[Δ1'[Δ2'[mrg'[agr1 agr2]]]]:=dyn_agree_ren_merge agr mrg.
+    have[Δ1'[Δ2'[mrg'[agr1 agr2]]]]:=program_agree_ren_merge agr mrg.
     have{}ihm:=ihm _ _ _ agr1.
     have{}ihn:=ihn _ _ _ agr2.
-    apply: era_app1...
+    apply: erasure_app1...
     asimpl in ihm... }
   { move=>Γ Δ A B m m' n t tyS tym ihm tyn Γ' Δ' ξ agr. asimpl.
     have{}ihm:=ihm _ _ _ agr.
-    have{}ihn:=sta_rename tyn (dyn_sta_agree_ren agr).
-    have{}ihS:=sta_rename tyS (dyn_sta_agree_ren agr).
-    apply: era_pair0...
+    have{}ihn:=logical_rename tyn (program_logical_agree_ren agr).
+    have{}ihS:=logical_rename tyS (program_logical_agree_ren agr).
+    apply: erasure_pair0...
     asimpl in ihS...
     asimpl. asimpl in ihn... }
   { move=>Γ Δ1 Δ2 Δ A B m m' n n' t mrg tyS tym ihm tyn ihn Γ' Δ' ξ agr. asimpl.
-    have[Δ1'[Δ2'[mrg'[agr1 agr2]]]]:=dyn_agree_ren_merge agr mrg.
+    have[Δ1'[Δ2'[mrg'[agr1 agr2]]]]:=program_agree_ren_merge agr mrg.
     have{}ihm:=ihm _ _ _ agr1.
     have{}ihn:=ihn _ _ _ agr2.
-    have{}ihS:=sta_rename tyS (dyn_sta_agree_ren agr).
-    apply: era_pair1...
+    have{}ihS:=logical_rename tyS (program_logical_agree_ren agr).
+    apply: erasure_pair1...
     asimpl in ihS...
     asimpl. asimpl in ihn... }
   { move=>Γ Δ1 Δ2 Δ A B C m m' n n' s r t mrg tyC tym ihm tyn ihn Γ' Δ' ξ agr. asimpl.
-    have wf:=sta_type_wf tyC. inv wf.
-    have wf:=dyn_type_wf (era_dyn_type tyn). inv wf. inv H4.
-    have[Δ1'[Δ2'[mrg'[agr1 agr2]]]]:=dyn_agree_ren_merge agr mrg.
-    have{}ihC:=sta_rename tyC (sta_agree_ren_cons H2 (dyn_sta_agree_ren agr)).
+    have wf:=logical_type_wf tyC. inv wf.
+    have wf:=program_type_wf (erasure_program_reflect tyn). inv wf. inv H4.
+    have[Δ1'[Δ2'[mrg'[agr1 agr2]]]]:=program_agree_ren_merge agr mrg.
+    have{}ihC:=logical_rename tyC (logical_agree_ren_cons H2 (program_logical_agree_ren agr)).
     have{}ihm:=ihm _ _ _ agr1.
-    have/ihn{}ihn:dyn_agree_ren (upren (upren ξ)) (B :: A :: Γ) (_: A :{r} Δ2)
+    have/ihn{}ihn:program_agree_ren (upren (upren ξ)) (B :: A :: Γ) (_: A :{r} Δ2)
       (B.[ren (upren ξ)] :: A.[ren ξ] :: Γ') (_: A.[ren ξ] :{r} Δ2')...
     asimpl in ihC.
     asimpl in ihm.
     replace C.[Pair0 (Var 1) (Var 0) t .: ren (+2)].[ren (upren (upren ξ))]
       with C.[ren (upren ξ)].[Pair0 (Var 1) (Var 0) t .: ren (+2)]
         in ihn by autosubst.
-    have:=era_letin0 mrg' ihC ihm ihn.
+    have:=erasure_letin0 mrg' ihC ihm ihn.
     by autosubst. }
   { move=>Γ Δ1 Δ2 Δ A B C m m' n n' s r1 r2 t mrg tyC tym ihm tyn ihn Γ' Δ' ξ agr. asimpl.
-    have wf:=sta_type_wf tyC. inv wf.
-    have wf:=dyn_type_wf (era_dyn_type tyn). inv wf. inv H4.
-    have[Δ1'[Δ2'[mrg'[agr1 agr2]]]]:=dyn_agree_ren_merge agr mrg.
-    have{}ihC:=sta_rename tyC (sta_agree_ren_cons H2 (dyn_sta_agree_ren agr)).
+    have wf:=logical_type_wf tyC. inv wf.
+    have wf:=program_type_wf (erasure_program_reflect tyn). inv wf. inv H4.
+    have[Δ1'[Δ2'[mrg'[agr1 agr2]]]]:=program_agree_ren_merge agr mrg.
+    have{}ihC:=logical_rename tyC (logical_agree_ren_cons H2 (program_logical_agree_ren agr)).
     have{}ihm:=ihm _ _ _ agr1.
-    have/ihn{}ihn:dyn_agree_ren (upren (upren ξ)) (B :: A :: Γ) (B :{r2} A :{r1} Δ2)
+    have/ihn{}ihn:program_agree_ren (upren (upren ξ)) (B :: A :: Γ) (B :{r2} A :{r1} Δ2)
       (B.[ren (upren ξ)] :: A.[ren ξ] :: Γ') (B.[ren (upren ξ)] :{r2} A.[ren ξ] :{r1} Δ2')...
     asimpl in ihC.
     asimpl in ihm.
     replace C.[Pair1 (Var 1) (Var 0) t .: ren (+2)].[ren (upren (upren ξ))]
       with C.[ren (upren ξ)].[Pair1 (Var 1) (Var 0) t .: ren (+2)]
         in ihn by autosubst.
-    have:=era_letin1 mrg' ihC ihm ihn.
+    have:=erasure_letin1 mrg' ihC ihm ihn.
     by autosubst. }
-  { move=>Γ Δ A B m m' n n' t k tym ihm tyn ihn Γ' Δ' ξ agr. asimpl. apply:era_apair... }
-  { move=>Γ Δ A B m m' t tym ihm Γ' Δ' ξ agr. asimpl. apply:era_fst... }
-  { move=>Γ Δ A B m m' t tym ihm Γ' Δ' ξ agr. asimpl. apply:era_snd... }
+  { move=>Γ Δ A B m m' n n' t k tym ihm tyn ihn Γ' Δ' ξ agr. asimpl. apply:erasure_apair... }
+  { move=>Γ Δ A B m m' t tym ihm Γ' Δ' ξ agr. asimpl. apply:erasure_fst... }
+  { move=>Γ Δ A B m m' t tym ihm Γ' Δ' ξ agr. asimpl. apply:erasure_snd... }
   { move=>Γ Δ A B H H' P m n s tyB erH ihH tyP Γ' Δ' ξ agr. asimpl.
-    have wf:=sta_type_wf tyB. inv wf. inv H2.
-    have ihP:=sta_rename tyP (dyn_sta_agree_ren agr).
-    have agr':=dyn_sta_agree_ren agr.
+    have wf:=logical_type_wf tyB. inv wf. inv H2.
+    have ihP:=logical_rename tyP (program_logical_agree_ren agr).
+    have agr':=program_logical_agree_ren agr.
     have{}agr':
-      sta_agree_ren (upren (upren ξ))
+      logical_agree_ren (upren (upren ξ))
         (Id A.[ren (+1)] m.[ren (+1)] (Var 0) :: A :: Γ)
         ((Id A.[ren (+1)] m.[ren (+1)] (Var 0)).[ren (upren ξ)] :: A.[ren ξ] :: Γ')...
-    have ihB:=sta_rename tyB agr'.
+    have ihB:=logical_rename tyB agr'.
     have{}ihH:=ihH _ _ _ agr.
     asimpl in ihP.
     asimpl in ihB.
     asimpl in ihH.
     replace A.[ren (ξ >>> (+1))] with A.[ren ξ].[ren (+1)] in ihB by autosubst.
     replace m.[ren (ξ >>> (+1))] with m.[ren ξ].[ren (+1)] in ihB by autosubst.
-    have pf:=era_rw ihB. asimpl in pf.
+    have pf:=erasure_rw ihB. asimpl in pf.
     have:=pf _ _ _ _ _ ihH ihP.
     by autosubst. }
   { move=>Γ Δ A B m m' s eq tym ihm tyB Γ' Δ' ξ agr.
-    apply: era_conv.
-    apply: sta_conv_subst...
+    apply: erasure_conv.
+    apply: logical_conv_subst...
     apply: ihm...
-    have:=sta_rename tyB (dyn_sta_agree_ren agr).
+    have:=logical_rename tyB (program_logical_agree_ren agr).
     asimpl... }
 Qed.
 
-Lemma era_weakenU Γ Δ m m' A B :
-  Γ ⊢ B : Sort U ->
-  Γ ; Δ ⊢ m ~ m' : A ->
-  (B :: Γ) ; B :U Δ ⊢ m.[ren (+1)] ~ m'.[ren (+1)] : A.[ren (+1)].
-Proof with eauto using dyn_agree_ren, dyn_agree_ren_refl.
-  move=>tyB tym. apply: era_rename...
-Qed.
-
-Lemma era_weakenN Γ Δ m m' A B s :
+(* Program 0-Weakening instrumented for erasure *)
+Lemma erasure_weaken0 Γ Δ m m' A B s :
   Γ ⊢ B : Sort s ->
   Γ ; Δ ⊢ m ~ m' : A ->
   (B :: Γ) ; _: Δ ⊢ m.[ren (+1)] ~ m'.[ren (+1)] : A.[ren (+1)].
-Proof with eauto using dyn_agree_ren, dyn_agree_ren_refl.
-  move=>tyB tym. apply: era_rename...
+Proof with eauto using program_agree_ren, program_agree_ren_refl.
+  move=>tyB tym. apply: erasure_rename...
 Qed.
 
-Lemma era_eweakenU Γ Δ m m' n n' A A' B :
-  m' = m.[ren (+1)] ->
-  n' = n.[ren (+1)] ->
-  A' = A.[ren (+1)] ->
+(* Program 1-Weakening instrumented for erasure *)
+Lemma erasure_weaken1 Γ Δ m m' A B :
   Γ ⊢ B : Sort U ->
-  Γ ; Δ ⊢ m ~ n : A ->
-  (B :: Γ) ; B :U Δ ⊢ m' ~ n' : A'.
-Proof.
-  move=>*; subst. exact: era_weakenU.
+  Γ ; Δ ⊢ m ~ m' : A ->
+  (B :: Γ) ; B :U Δ ⊢ m.[ren (+1)] ~ m'.[ren (+1)] : A.[ren (+1)].
+Proof with eauto using program_agree_ren, program_agree_ren_refl.
+  move=>tyB tym. apply: erasure_rename...
 Qed.
 
-Lemma era_eweakenN Γ Δ m m' n n' A A' B s :
+(* Alternative statement more suitable for certain Coq tactics *)
+Lemma erasure_eweaken0 Γ Δ m m' n n' A A' B s :
   m' = m.[ren (+1)] ->
   n' = n.[ren (+1)] ->
   A' = A.[ren (+1)] ->
@@ -148,5 +144,17 @@ Lemma era_eweakenN Γ Δ m m' n n' A A' B s :
   Γ ; Δ ⊢ m ~ n : A ->
   (B :: Γ) ; (_: Δ) ⊢ m' ~ n' : A'.
 Proof.
-  move=>*; subst. apply: era_weakenN; eauto.
+  move=>*; subst. apply: erasure_weaken0; eauto.
+Qed.
+
+(* Alternative statement more suitable for certain Coq tactics *)
+Lemma erasure_eweaken1 Γ Δ m m' n n' A A' B :
+  m' = m.[ren (+1)] ->
+  n' = n.[ren (+1)] ->
+  A' = A.[ren (+1)] ->
+  Γ ⊢ B : Sort U ->
+  Γ ; Δ ⊢ m ~ n : A ->
+  (B :: Γ) ; B :U Δ ⊢ m' ~ n' : A'.
+Proof.
+  move=>*; subst. exact: erasure_weaken1.
 Qed.
