coq/theories/program_inv.v
@@ -1,12 +1,14 @@
+(* The file presents various inversion lemmas for the program level. *)
+
 From mathcomp Require Import ssreflect ssrbool eqtype ssrnat seq.
 From Coq Require Import ssrfun Classical Utf8.
-Require Export AutosubstSsr ARS sta_uniq sta_sr dyn_subst.
+Require Export AutosubstSsr ARS logical_uniq logical_sr program_subst.
 
 Set Implicit Arguments.
 Unset Strict Implicit.
 Unset Printing Implicit Defensive.
 
-Lemma dyn_lam0_invX Γ Δ A1 A2 B C m s1 s2 t :
+Lemma program_lam0_invX Γ Δ A1 A2 B C m s1 s2 t :
   Γ ; Δ ⊢ Lam0 A1 m s1 : C ->
   C === Pi0 A2 B s2 ->
   (A2 :: Γ) ⊢ B : Sort t ->
@@ -16,20 +18,20 @@ Proof with eauto.
   elim: tyL A1 A2 B m s1 s2 t e=>//{Γ Δ C n}.
   { move=>Γ Δ A B m s k tym _ A1 A2 B0 m0
       s1 s2 t[e1 e2 e3]/pi0_inj[eq1[eq2 e4]]tyB0; subst.
-    have wf:=dyn_type_wf tym. inv wf.
-    have wf:=sta_type_wf tyB0. inv wf.
-    apply: dyn_ctx_conv0.
+    have wf:=program_type_wf tym. inv wf.
+    have wf:=logical_type_wf tyB0. inv wf.
+    apply: program_ctx_conv0.
     apply: conv_sym...
     exact: H4.
-    apply: dyn_conv...
-    apply: sta_ctx_conv... }
+    apply: program_conv...
+    apply: logical_ctx_conv... }
   { move=>Γ Δ A B m s eq tym ihm tyB A1 A2 B0 m0
       s1 s2 t e eq2 tyB0; subst.
     apply: ihm...
     apply: conv_trans... }
 Qed.
 
-Lemma dyn_lam1_invX Γ Δ A1 A2 B C m s1 s2 t :
+Lemma program_lam1_invX Γ Δ A1 A2 B C m s1 s2 t :
   Γ ; Δ ⊢ Lam1 A1 m s1 : C ->
   C === Pi1 A2 B s2 ->
   (A2 :: Γ) ⊢ B : Sort t ->
@@ -39,41 +41,41 @@ Proof with eauto.
   elim: tyL A1 A2 B m s1 s2 t e=>//{Γ Δ C n}.
   { move=>Γ Δ A B m s t k tym _ A1 A2 B0 m0
       s1 s2 t0[e1 e2 e3]/pi1_inj[eq1[eq2 e4]]tyB0; subst.
-    have wf:=dyn_type_wf tym. inv wf.
-    have wf:=sta_type_wf tyB0. inv wf.
+    have wf:=program_type_wf tym. inv wf.
+    have wf:=logical_type_wf tyB0. inv wf.
     have[A0 rd1 rd2]:=church_rosser eq1.
-    have tyA0t:=sta_rd H4 rd1.
-    have tyA0s:=sta_rd H3 rd2.
-    have e:=sta_unicity tyA0t tyA0s. subst.
+    have tyA0t:=logical_rd H4 rd1.
+    have tyA0s:=logical_rd H3 rd2.
+    have e:=logical_sort_uniq tyA0t tyA0s. subst.
     exists s.
-    apply: dyn_ctx_conv1.
+    apply: program_ctx_conv1.
     apply: conv_sym...
     exact: H3.
-    apply: dyn_conv...
-    apply: sta_ctx_conv... }
+    apply: program_conv...
+    apply: logical_ctx_conv... }
   { move=>Γ Δ A B m s eq tym ihm tyB A1 A2 B0 m0
       s1 s2 t e eq2 tyB0; subst.
     apply: ihm...
     apply: conv_trans... }
 Qed.
 
-Lemma dyn_lam0_inv Γ Δ m A1 A2 B s1 s2 :
+Lemma program_lam0_inv Γ Δ m A1 A2 B s1 s2 :
   Γ ; Δ ⊢ Lam0 A2 m s2 : Pi0 A1 B s1 -> (A1 :: Γ) ; _: Δ ⊢ m : B.
 Proof with eauto.
   move=>ty.
-  have[t/sta_pi0_inv[r[tyB _]]]:=dyn_valid ty.
-  apply: dyn_lam0_invX...
+  have[t/logical_pi0_inv[r[tyB _]]]:=program_valid ty.
+  apply: program_lam0_invX...
 Qed.
 
-Lemma dyn_lam1_inv Γ Δ m A1 A2 B s1 s2 :
+Lemma program_lam1_inv Γ Δ m A1 A2 B s1 s2 :
   Γ ; Δ ⊢ Lam1 A2 m s2 : Pi1 A1 B s1 -> exists r, (A1 :: Γ) ; A1 :{r} Δ ⊢ m : B.
 Proof with eauto.
   move=>ty.
-  have[t/sta_pi1_inv[r[tyB _]]]:=dyn_valid ty.
-  apply: dyn_lam1_invX...
+  have[t/logical_pi1_inv[r[tyB _]]]:=program_valid ty.
+  apply: program_lam1_invX...
 Qed.
 
-Lemma dyn_pair0_invX Γ Δ A B m n s r t C :
+Lemma program_pair0_invX Γ Δ A B m n s r t C :
   Γ ; Δ ⊢ Pair0 m n s : C ->
   C === Sig0 A B r ->
   Γ ⊢ Sig0 A B r : Sort t ->
@@ -83,20 +85,20 @@ Proof with eauto.
   elim: ty A B m n s r t e=>//{Γ Δ x C}.
   { move=>Γ Δ A B m n t ty1 tym ihm tyn A0 B0 m0 n0 s r t0[e1 e2 e3]
       /sig0_inj[e4[e5 e6]]ty2; subst.
-    have[s[r0[ord[tyA0[tyB0/sort_inj e]]]]]:=sta_sig0_inv ty2. subst.
-    have tym0:Γ ; Δ ⊢ m : A0 by apply: dyn_conv; eauto.
+    have[s[r0[ord[tyA0[tyB0/sort_inj e]]]]]:=logical_sig0_inv ty2. subst.
+    have tym0:Γ ; Δ ⊢ m : A0 by apply: program_conv; eauto.
     repeat split...
-    apply: sta_conv.
-    apply: sta_conv_subst.
+    apply: logical_conv.
+    apply: logical_conv_subst.
     all: eauto.
-    apply: sta_esubst...
+    apply: logical_esubst...
     by autosubst. }
   { move=>Γ Δ A B m s eq tym ihm tyB A0 B0 m0 n s0 r t e eq' ty.
     apply: ihm...
     apply: conv_trans... }
 Qed.
 
-Lemma dyn_pair1_invX Γ Δ A B m n s r t C :
+Lemma program_pair1_invX Γ Δ A B m n s r t C :
   Γ ; Δ ⊢ Pair1 m n s : C ->
   C === Sig1 A B r ->
   Γ ⊢ Sig1 A B r : Sort t ->
@@ -109,40 +111,40 @@ Proof with eauto.
   { move=>Γ Δ1 Δ2 Δ A B m n t mrg ty1 tym _ tyn _ A0 B0 m0 n0 s r t0
       [e1 e2 e3]/sig1_inj[e4[e5 e6]]ty2; subst.
     exists Δ1. exists Δ2.
-    have[s[r0[ord1[ord2[tyA0[tyB0/sort_inj e]]]]]]:=sta_sig1_inv ty2. subst.
-    have tym0:Γ ; Δ1 ⊢ m : A0 by apply: dyn_conv; eauto.
+    have[s[r0[ord1[ord2[tyA0[tyB0/sort_inj e]]]]]]:=logical_sig1_inv ty2. subst.
+    have tym0:Γ ; Δ1 ⊢ m : A0 by apply: program_conv; eauto.
     repeat split...
-    apply: dyn_conv.
-    apply: sta_conv_subst.
+    apply: program_conv.
+    apply: logical_conv_subst.
     all: eauto.
-    apply: sta_esubst...
+    apply: logical_esubst...
     by autosubst. }
   { move=>Γ Δ A B m s eq tym ihm tyB A0 B0 m0 n s0 r t e eq' ty.
     apply: ihm...
     apply: conv_trans... }
 Qed.
 
-Lemma dyn_pair0_inv Γ Δ A B m n s r :
+Lemma program_pair0_inv Γ Δ A B m n s r :
   Γ ; Δ ⊢ Pair0 m n s : Sig0 A B r ->
   s = r /\ Γ ; Δ ⊢ m : A /\ Γ ⊢ n : B.[m/].
 Proof with eauto.
   move=>ty.
-  have[t tyS]:=dyn_valid ty.
-  apply: dyn_pair0_invX...
+  have[t tyS]:=program_valid ty.
+  apply: program_pair0_invX...
 Qed.
 
-Lemma dyn_pair1_inv Γ Δ A B m n s r :
+Lemma program_pair1_inv Γ Δ A B m n s r :
   Γ ; Δ ⊢ Pair1 m n s : Sig1 A B r ->
   exists Δ1 Δ2,
     Δ1 ∘ Δ2 => Δ /\ s = r /\
     Γ ; Δ1 ⊢ m : A /\ Γ ; Δ2 ⊢ n : B.[m/].
 Proof with eauto.
   move=>ty.
-  have[t tyS]:=dyn_valid ty.
-  apply: dyn_pair1_invX...
+  have[t tyS]:=program_valid ty.
+  apply: program_pair1_invX...
 Qed.
 
-Lemma dyn_apair_invX Γ Δ A B m n s r t C :
+Lemma program_apair_invX Γ Δ A B m n s r t C :
   Γ ; Δ ⊢ APair m n s : C ->
   C === With A B r ->
   Γ ⊢ With A B r : Sort t ->
@@ -152,20 +154,20 @@ Proof with eauto.
   elim: ty A B m n s r t e=>//{Γ Δ x C}.
   { move=>Γ Δ A B m n t k tym ihm tyn ihn A0 B0 m0 n0 s r t0
       [e1 e2 e3]/with_inj[e4[e5 e6]]ty; subst.
-    have[s[r0[tyA0[tyB0 _]]]]:=sta_with_inv ty.
+    have[s[r0[tyA0[tyB0 _]]]]:=logical_with_inv ty.
     repeat split...
-    apply: dyn_conv...
-    apply: dyn_conv... }
+    apply: program_conv...
+    apply: program_conv... }
   { move=>Γ Δ A B m s eq tym ihm _ A0 B0 m0 n s0 r t e eq' tyw; subst.
     apply: ihm...
     apply: conv_trans... }
 Qed.
 
-Lemma dyn_apair_inv Γ Δ A B m n s r :
+Lemma program_apair_inv Γ Δ A B m n s r :
   Γ ; Δ ⊢ APair m n s : With A B r ->
   s = r /\ Γ ; Δ ⊢ m : A /\ Γ ; Δ ⊢ n : B.
 Proof with eauto.
   move=>ty.
-  have[t tyW]:=dyn_valid ty.
-  apply: dyn_apair_invX...
+  have[t tyW]:=program_valid ty.
+  apply: program_apair_invX...
 Qed.
