coq/theories/program_prog.v
@@ -1,24 +1,27 @@
+(* This file presents the program level progress theorem and various
+   canonical forms lemmas necessary to prove it. *)
+
 From mathcomp Require Import ssreflect ssrbool eqtype ssrnat seq.
 From Coq Require Import ssrfun Classical Utf8.
-Require Export AutosubstSsr ARS sta_sr dyn_sr.
+Require Export AutosubstSsr ARS logical_sr program_sr.
 
 Set Implicit Arguments.
 Unset Strict Implicit.
 Unset Printing Implicit Defensive.
 
-Ltac inv_dyn_val :=
+Ltac inv_program_val :=
   match goal with
-  | [ H : dyn_val _ |- _ ] => inv H
+  | [ H : program_val _ |- _ ] => inv H
   end.
 
-Lemma dyn_pi0_canonical m A B C s :
-  nil ; nil ⊢ m : C -> C === Pi0 A B s -> dyn_val m ->
+Lemma program_pi0_canonical m A B C s :
+  nil ; nil ⊢ m : C -> C === Pi0 A B s -> program_val m ->
   exists A n, m = Lam0 A n s.
 Proof with eauto.
   move e1:(nil)=>Γ.
   move e2:(nil)=>Δ ty.
   elim: ty A B s e1 e2=>//{Γ Δ m C}.
-  all: try solve[intros; exfalso; (solve_conv||inv_dyn_val)].
+  all: try solve[intros; exfalso; (solve_conv||inv_program_val)].
   { move=>Γ Δ x s A wf shs dhs A0 B s0 e1 e2; subst. inv shs. }
   { move=>Γ Δ A B m s k tym ihm A0 B0 s0
       e1 e2/pi0_inj[eq1[eq2 e3]] vl; subst.
@@ -28,14 +31,14 @@ Proof with eauto.
     apply: conv_trans... }
 Qed.
 
-Lemma dyn_pi1_canonical m A B C s :
-  nil ; nil ⊢ m : C -> C === Pi1 A B s -> dyn_val m ->
+Lemma program_pi1_canonical m A B C s :
+  nil ; nil ⊢ m : C -> C === Pi1 A B s -> program_val m ->
   exists A n, m = Lam1 A n s.
 Proof with eauto.
   move e1:(nil)=>Γ.
   move e2:(nil)=>Δ ty.
   elim: ty A B s e1 e2=>//{Γ Δ m C}.
-  all: try solve[intros; exfalso; (solve_conv||inv_dyn_val)].
+  all: try solve[intros; exfalso; (solve_conv||inv_program_val)].
   { move=>Γ Δ x s A wf shs dhs A0 B s0 e1 e2; subst. inv shs. }
   { move=>Γ Δ A B m s t k tym ihm A0 B0 s0
       e1 e2/pi1_inj[eq1[eq2 e3]] vl; subst.
@@ -45,14 +48,14 @@ Proof with eauto.
     apply: conv_trans... }
 Qed.
 
-Lemma dyn_sig0_canonical m A B C s :
-  nil ; nil ⊢ m : C -> C === Sig0 A B s -> dyn_val m ->
+Lemma program_sig0_canonical m A B C s :
+  nil ; nil ⊢ m : C -> C === Sig0 A B s -> program_val m ->
   exists m1 m2, m = Pair0 m1 m2 s.
 Proof with eauto.
   move e1:(nil)=>Γ.
   move e2:(nil)=>Δ ty.
   elim: ty A B s e1 e2=>//{Γ Δ m C}.
-  all: try solve[intros; exfalso; (solve_conv||inv_dyn_val)].
+  all: try solve[intros; exfalso; (solve_conv||inv_program_val)].
   { move=>Γ Δ x s A wf shs dhs A0 B s0 e1 e2; subst. inv shs. }
   { move=>Γ Δ A B m n t tyS tym ihm tyn A0 B0 s
       e1 e2/sig0_inj[eq1[eq2 e3]] vl; subst.
@@ -62,14 +65,14 @@ Proof with eauto.
     apply: conv_trans... }
 Qed.
 
-Lemma dyn_sig1_canonical m A B C s :
-  nil ; nil ⊢ m : C -> C === Sig1 A B s -> dyn_val m ->
+Lemma program_sig1_canonical m A B C s :
+  nil ; nil ⊢ m : C -> C === Sig1 A B s -> program_val m ->
   exists m1 m2, m = Pair1 m1 m2 s.
 Proof with eauto.
   move e1:(nil)=>Γ.
   move e2:(nil)=>Δ ty.
   elim: ty A B s e1 e2=>//{Γ Δ m C}.
-  all: try solve[intros; exfalso; (solve_conv||inv_dyn_val)].
+  all: try solve[intros; exfalso; (solve_conv||inv_program_val)].
   { move=>Γ Δ x s A wf shs dhs A0 B s0 e1 e2; subst. inv shs. }
   { move=>Γ Δ1 Δ2 Δ A B m n t mrg tyS tym ihm tyn ihn A0 B0 s
       e1 e2/sig1_inj[eq1[eq2 e3]]vl; subst.
@@ -79,14 +82,14 @@ Proof with eauto.
     apply: conv_trans... }
 Qed.
 
-Lemma dyn_with_canonical m A B C s :
-  nil ; nil ⊢ m : C -> C === With A B s -> dyn_val m ->
+Lemma program_with_canonical m A B C s :
+  nil ; nil ⊢ m : C -> C === With A B s -> program_val m ->
   exists m1 m2, m = APair m1 m2 s.
 Proof with eauto.
   move e1:(nil)=>Γ.
   move e2:(nil)=>Δ ty.
   elim: ty A B s e1 e2=>//{Γ Δ m C}.
-  all: try solve[intros; exfalso; (solve_conv||inv_dyn_val)].
+  all: try solve[intros; exfalso; (solve_conv||inv_program_val)].
   { move=>Γ Δ x s A wf shs dhs A0 B s0 e1 e2; subst. inv shs. }
   { move=>Γ Δ A B m n t k tym ihm tyn ihn A0 B0 s
       e1 e2/with_inj[eq1[eq2 e3]]vl; subst.
@@ -96,8 +99,9 @@ Proof with eauto.
     apply: conv_trans... }
 Qed.
 
-Lemma dyn_prog m A : nil ; nil ⊢ m : A -> (exists n, m ~>> n) \/ dyn_val m.
-Proof with eauto using dyn_step, dyn_val.
+(* Theorem 9 (Program Progress) *)
+Lemma program_prog m A : nil ; nil ⊢ m : A -> (exists n, m ~>> n) \/ program_val m.
+Proof with eauto using program_step, program_val.
   move e1:(nil)=>Γ.
   move e2:(nil)=>Δ ty. elim: ty e1 e2=>{Γ Δ m A}.
   { move=>Γ Δ x s A wf shs dhs e1 e2; subst. inv shs. }
@@ -109,14 +113,14 @@ Proof with eauto using dyn_step, dyn_val.
     have[[x st]|vl]:=ihm erefl erefl.
     { left. exists (App x n)... }
     { left.
-      have[A0[n0 e]]:=dyn_pi0_canonical tym (convR _ _) vl.
+      have[A0[n0 e]]:=program_pi0_canonical tym (convR _ _) vl.
       subst. exists (n0.[n/])... } }
   { move=>Γ Δ1 Δ2 Δ A B m n s mrg tym ihm tyn ihn e1 e2; subst.
     inv mrg. have[[m' stm]|vlm]:=ihm erefl erefl.
     { left. exists (App m' n)... }
     { left. have[[n' stn]|vln]:=ihn erefl erefl.
       exists (App m n')...
-      have[A0[n0 e]]:=dyn_pi1_canonical tym (convR _ _) vlm.
+      have[A0[n0 e]]:=program_pi1_canonical tym (convR _ _) vlm.
       subst. exists (n0.[n/])... } }
   { move=>Γ Δ A B m n t tyS tym ihm tyn e1 e2; subst.
     have[[m' stm]|vlm]:=ihm erefl erefl.
@@ -132,23 +136,23 @@ Proof with eauto using dyn_step, dyn_val.
   { move=>Γ Δ1 Δ2 Δ A B C m n s r t mrg tyC tym ihm tyn ihn e1 e2; subst.
     inv mrg. have[[m' stm]|vlm]:=ihm erefl erefl.
     { left. exists (LetIn C m' n)... }
-    { have[m1[m2 e]]:=dyn_sig0_canonical tym (convR _ _) vlm. subst.
+    { have[m1[m2 e]]:=program_sig0_canonical tym (convR _ _) vlm. subst.
       left. exists n.[m2,m1/]... } }
   { move=>Γ Δ1 Δ2 Δ A B C m n s r1 r2 t mrg tyC tym ihm tyn ihn e1 e2; subst.
     inv mrg. have[[m' stm]|vlm]:=ihm erefl erefl.
     { left. exists (LetIn C m' n)... }
-    { have[m1[m2 e]]:=dyn_sig1_canonical tym (convR _ _) vlm. subst.
+    { have[m1[m2 e]]:=program_sig1_canonical tym (convR _ _) vlm. subst.
       left. exists n.[m2,m1/]... } }
   { move=>Γ Δ A B m n t k tym ihm tyn ihn e1 e2; subst. right... }
   { move=>Γ Δ A B m t tym ihm e1 e2; subst.
     have[[m' stm]|vlm]:=ihm erefl erefl.
     { left. exists (Fst m')... }
-    { have[m1[m2 e]]:=dyn_with_canonical tym (convR _ _) vlm. subst.
+    { have[m1[m2 e]]:=program_with_canonical tym (convR _ _) vlm. subst.
       left. exists m1... } }
   { move=>Γ Δ A B m t tym ihm e1 e2; subst.
     have[[m' stm]|vlm]:=ihm erefl erefl.
     { left. exists (Snd m')... }
-    { have[m1[m2 e]]:=dyn_with_canonical tym (convR _ _) vlm. subst.
+    { have[m1[m2 e]]:=program_with_canonical tym (convR _ _) vlm. subst.
       left. exists m2... } }
   { move=>Γ Δ A B H P m n s tyB tyH ihH tyP e1 e2. subst.
     left. exists H... }
